@prefix : <http://onto.mtconnect.org/ontologies/mtconnect#> .
@prefix owl: <http://www.w3.org/2002/07/owl#> .
@prefix rdf: <http://www.w3.org/1999/02/22-rdf-syntax-ns#> .
@prefix xml: <http://www.w3.org/XML/1998/namespace> .
@prefix xsd: <http://www.w3.org/2001/XMLSchema#> .
@prefix rdfs: <http://www.w3.org/2000/01/rdf-schema#> .
@prefix ssn: <http://www.w3.org/ns/ssn/> .
@prefix sosa: <http://www.w3.org/ns/ssn/> .
@prefix skos: <http://www.w3.org/2008/05/skos#> .
@prefix sosa: <http://www.w3.org/ns/sosa/> .
@prefix time: <http://www.w3.org/2006/time#> .
@prefix schema: <http://schema.org/> .
@base <http://onto.mtconnect.org/ontologies/mtconnect> .

<http://onto.mtconnect.org/ontologies/mtconnect> rdf:type owl:Ontology ;
    owl:versionIRI <http://onto.mtconnect.org/ontologies/mtconnect/2019/08/0.1.0> ;
    owl:imports <http://www.w3.org/2006/time#2016> ,
    <http://www.w3.org/ns/ssn/>, <http://www.w3.org/2008/05/skos> .

# Observable Properties

:hasObservation a owl:ObjectProperty ;
    rdfs:domain :Observable ;
    rdfs:range :Observation .

:uses a owl:ObjectProperty ;
    rdfs:domain :Observable ;
    rdfs:range :Procedure .

:madeForObservable a owl:ObjectProperty ;
    rdfs:domain :Observation ;
    rdfs:range :Observable ;
    owl:inverseOf :hasObservation .
    
:canObserve a owl:ObjectProperty ;
    rdfs:comment "Something that can observing something else" .

## Specific relationships by category. The subproperties allow for the
## associations to be typed even when they overlap.

:canObserveSample a owl:ObjectProperty ;
    rdfs:range :Sample ;
    rdfs:subPropertyOf :canObserve .

:canObserveEvent a owl:ObjectProperty ;
    rdfs:range :Event ;
    rdfs:subPropertyOf :canObserve .
    
:canObserveCondition a owl:ObjectProperty ;
    rdfs:range :Condition ;
    rdfs:subPropertyOf :canObserve .
    
:canObserveState a owl:ObjectProperty ;
    rdfs:range :State ;
    rdfs:subPropertyOf :canObserve .
    
:isObservable a owl:ObjectProperty ;
    owl:inverseOf :canObserve .
    
# Component Properties

:madeObservation a owl:ObjectProperty ;
    rdfs:range :Observation .
    
:observedBy a owl:ObjectProperty ;
    rdfs:domain :Observation ;
    owl:inverseOf :madeObservation ;
    rdfs:comment "The  thing that was made the observation" .

:subjectOf a owl:ObjectProperty ;
    rdfs:domain :Observation ;
    owl:equivalentProperty sosa:hasFeatureOfInterest ;
    rdfs:comment "The thing that is being observed by the observation" .
    
# Classes

# Component Base

:Component a owl:Class ;
           rdfs:comment """A Component comprises a logical part of a Device and provides observations about the Component as DataItems. The Component has the Characteristics and Capabilities of the Component that composed to the overall Capabilities of the machine.

In MTConnect, a Composition further decomposes the Component into various atomic units that cannot be decomposed further. The Composition adds additional context to the DataItem regarding the source of the data. For example, a Linear axis will have a Motor and an Amplifier that are represented as Compositions. The Motor and Amplifier can both have a DataItem that reports their respective Temperature."""@en ;
    rdfs:subClassOf ssn:System .

:Device a owl:Class ;
    rdfs:subClassOf :Component ;
    rdfs:comment "A Device is a System that represents a machine used in a manufacturing process. A Device is composed of Components through the transitive has components relationship. The Device definition derives from the MTConnect Standard." .
    
# Observable
    
:Observable a owl:Class ;
    rdfs:comment "Equivalent an ObservableProperty, but also providing an individual to describe something that is observable by an Entity and can provide data. The Observable provides the properties about the thing being observed." ;    
    owl:equivalentClass sosa:ObservableProperty ;
    rdfs:subClassOf [ a owl:Restriction ; owl:onProperty :isObservable ; owl:allValuesFrom :Component ] .

:DataItem a owl:Class ;
    rdfs:comment "The DataItem is somethings that is Observable of the Component and provides the Meta Data associated with the DataItem. The DataItem properties include units, native units, and representation" ;    
    rdfs:subClassOf :Observable .
    
:Sample a owl:Class ;
    rdfs:comment "An MTConnect sampled value that is a point in time reading from a sensor or control system. Samples are continuous variables that allow for the computation of intermediate values. For Observable Samples with a statistic, the TemporalEntity represents an interval derived from the MTConnect timestamp and the duration." ;    
    rdfs:subClassOf :DataItem .
    
:State a owl:Class ;
    rdfs:comment "MTConnect does not differentiate between State and Event, but the ontology classifies all MTConnect Event category Data Items with controlled vocabularies (finite range) referencing a set of individuals representing the allowable states." ;    
    rdfs:subClassOf :DataItem .
    
:Event a owl:Class ;
    rdfs:comment "For Data Items with the category EVENT and an unlimited range, like a program name or a message as specified by an xsd:string type, the Event type is used." ;    
    rdfs:subClassOf :DataItem .

:Condition a owl:Class ;
    rdfs:comment "The MTConnect condition provides the faults or warnings related to some aspect of the component. A Fault occurs when the machine requires manual intervention to fix and issue and a Warning indicates the machine is trending towards a Fault, but can still operate and measures should be taken to prevent a failure. The Condition has multiple properties as defined in the MTConnect standard." ;    
    rdfs:subClassOf :DataItem .

:Constraint rdf:type owl:Class .

[ rdf:type owl:AllDisjointClasses ;
        owl:members ( :Sample
            :State
            :Event
            :Condition
            )
        ] .


# Observation

:Observation a owl:Class ;
    rdfs:comment "An Observation is a set of Results that share the same temporal space and may be associated with something Observable. The individual Observation is an instance of when something occurs in the manufacturing environment at a point in time or over an interval." ;
    owl:equivalentClass sosa:Observation .
        
:Result a owl:Class ;
    rdfs:comment "A Result is a value given by the Observation that has more than a single data propert, such as a Conditon Warning or Fault. " ;
    owl:equivalentClass sosa:Result .    

:ConditionState a owl:Class ;
    rdfs:subClassOf :Result .

:Fault a owl:Class ;
    rdfs:subClassOf :ConditionState .
    
:Warning a owl:Class ;
    rdfs:subClassOf :ConditionState .
    
:Normal a owl:Class ;
    rdfs:subClassOf :ConditionState .
    
# Procedure

:Procedure a owl:Class .

# Properties

# Component properties

:hasComponent a owl:ObjectProperty, owl:TransitiveProperty ;
    rdfs:domain :Component ;
    rdfs:range :Component .    

:componentOf a owl:ObjectProperty ;
    owl:inverseOf :hasComponent ;
    rdfs:domain :Component ;
    rdfs:range :Component .

:hasConfiguration a owl:ObjectProperty ;
    rdfs:domain :Component ;
    rdfs:range :Configuration .
    
:configurationFor a owl:ObjectProperty ;
    owl:inverseOf :hasConfiguration ;
    rdfs:domain :Configuration ;
    rdfs:range :Component .

:hasUuid a owl:DatatypeProperty ,
        owl:FunctionalProperty ;        
    rdfs:domain :Component ;
    rdfs:range xsd:string .

:hasSerialNumber a owl:DatatypeProperty ,
        owl:FunctionalProperty ;        
    rdfs:domain :Component ;
    rdfs:range xsd:string .

:hasName a owl:DatatypeProperty,
        owl:FunctionalProperty ;
    rdf:type owl:FunctionalProperty ;
    rdfs:domain :Component ,
        :DataItem ;
    rdfs:range xsd:string .

:hasNativeName a owl:DatatypeProperty ,
        owl:FunctionalProperty ;
    rdfs:domain :Component ;
    rdfs:range xsd:string .


:hasManufacturer a owl:DatatypeProperty ,
        owl:FunctionalProperty ;
    rdfs:domain :Component ;
    rdfs:range xsd:string .

:hasXmlId a owl:DatatypeProperty ,
        owl:FunctionalProperty ;
    rdfs:domain :Component , :DataItem ;
    rdfs:range xsd:string .

:hasDescription a owl:DatatypeProperty ,
        owl:FunctionalProperty ;
    rdfs:domain :Component ;
    rdfs:range xsd:string .

# Data Item properties

:hasDataItem a owl:ObjectProperty ;
    rdfs:domain :Component ;
    rdfs:range :DataItem .

:hasConstraint a owl:ObjectProperty ,
        owl:FunctionalProperty ;
    rdfs:domain :DataItem ;
    rdfs:range :Constraint .


:hasSource a owl:ObjectProperty ;
    rdfs:domain :DataItem ;    
    rdf:type owl:FunctionalProperty .

:isSourceOf a owl:ObjectProperty ,
        owl:InverseFunctionalProperty ;
    rdfs:range :DataItem ;    
    owl:inverseOf :hasSource .

:hasUnit a owl:ObjectProperty ;
    rdfs:domain :DataItem ;
    rdfs:range :Unit .

# Observation Properties

## Simple Properties

:hasValue a owl:DatatypeProperty .

:hasSampledValue a owl:DatatypeProperty ;
    rdfs:subPropertyOf :hasValue ;
    owl:equivalentProperty sosa:hasSimpleResult ;    
    rdfs:range xsd:float .

:hasEventValue a owl:DatatypeProperty ;
    rdfs:subPropertyOf :hasValue ;
    rdfs:range xsd:float .

:hasState a owl:ObjectProperty .

# Timestamps

:period a owl:ObjectProperty ;
    owl:equivalentProperty sosa:phenomenonTime ;
    rdfs:domain :Observation ;
    rdfs:range time:TemporalEntity .
    
:timestamp a owl:DatatypeProperty ;
    rdfs:domain :Observation ;
    rdfs:range xsd:dateTime .

:hasResult a owl:ObjectProperty ;
    rdfs:domain :Observation ;
    rdfs:range :Result .

# Condition State properties

:hasNativeCode a owl:DatatypeProperty ;
    rdfs:domain :ConditionState ;
    rdfs:range xsd:string .
    
:hasNativeSeverity a owl:DatatypeProperty ;
    rdfs:domain :ConditionState ;
    rdfs:range xsd:string .

:Qualifier a owl:Class ;
    owl:equivalentClass [ owl:intersectionOf ( owl:Thing
            [ rdf:type owl:Class ;
                owl:oneOf ( :HIGH :LOW )
                ]
            ) ;
        ] .

:hasQualifier a owl:ObjectProperty ;
    rdfs:domain :ConditionState ;
    rdfs:range :Qualifier .    

[ rdf:type owl:AllDisjointClasses ;
        owl:members ( :Component
            :Result
            :Observable
            :Observation
            :Procedure
            :Constraint
            )
        ] .
        
# ---------------------------------------------------------------------------------------
# Generated code
# ---------------------------------------------------------------------------------------

:Unit a owl:Class ;
    owl:equivalentClass [ owl:intersectionOf ( owl:Thing 
            [ rdf:type owl:Class ;
                owl:oneOf (
                    :AMPERE
                    :CELSIUS
                    :COUNT
                    :DECIBEL
                    :DEGREE
                    :DEGREE_PER_SECOND
                    :DEGREE_PER_SECOND_SQ
                    :HERTZ
                    :JOULE
                    :KILOGRAM
                    :LITER
                    :LITER_PER_SECOND
                    :MICRO_RADIAN
                    :MILLIMETER
                    :MILLIMETER_3D
                    :MILLIMETER_PER_REVOLUTION
                    :MILLIMETER_PER_SECOND
                    :MILLIMETER_PER_SECOND_SQ
                    :NEWTON
                    :NEWTON_METER
                    :OHM
                    :PASCAL
                    :PASCAL_SECOND
                    :PERCENT
                    :PH
                    :REVOLUTION_PER_MINUTE
                    :SECOND
                    :SIEMENS_PER_METER
                    :VOLT
                    :VOLT_AMPERE
                    :VOLT_AMPERE_REACTIVE
                    :WATT
                    :WATT_SECOND
                    )
                ]
            ) ;
            a owl:Class
        ] .
:Actuator a owl:Class ;
	rdfs:subClassOf :Component ;
	rdfs:comment "Redefined as a piece of equipment with the ability to be represented as a lower level component of a parent component element or as a composition element. See actuator type"@en .

:Auxiliaries a owl:Class ;
	rdfs:subClassOf :Component ;
	rdfs:comment "An XML container used to organize information for lower level elements representing functional sub-systems that provide supplementary or extended capabilities for a piece of equipment, but they are not required for the basic operation of the equipment."@en .

:Axes a owl:Class ;
	rdfs:subClassOf :Component ;
	rdfs:comment "An XML container used to organize the structural element of a piece of equipment that perform linear or rotational motion."@en .

:BarFeeder a owl:Class ;
	rdfs:subClassOf :Auxiliaries ;
	rdfs:comment "barfeeder is an XML container that represents the information for a unit involved in delivering bar stock to a piece of equipment."@en .

:Chuck a owl:Class ;
	rdfs:subClassOf :Rotary ;
	rdfs:comment "Chuck is an XML container that provides the information about a mechanism that holds a part or stock material in place."@en .

:Controller a owl:Class ;
	rdfs:subClassOf :Component ;
	rdfs:comment "An XML container used to organize information about an intelligent or computational function within a piece of equipment."@en .

:Coolant a owl:Class ;
	rdfs:subClassOf :Systems ;
	rdfs:comment "coolant is an XML container that represents the information for a system comprised of all the parts involved in distribution and management of fluids that remove heat from a piece of equipment."@en .

:Deposition a owl:Class ;
	rdfs:subClassOf :Component ;
	rdfs:comment "deposition is an XML container that represents the information for a system that manages the addition of material or state change of material being performed in an additive manufacturing process.  For example, this could describe the portion of a piece of equipment that manages a material extrusion process or a vat polymerization process."@en .

:Dielectric a owl:Class ;
	rdfs:subClassOf :Systems ;
	rdfs:comment "dielectric is an XML container that represents the information for a system that manages a chemical mixture used in a manufacturing process being performed at that piece of equipment."@en .

:Door a owl:Class ;
	rdfs:subClassOf :Component ;
	rdfs:comment "door component is an XML container that represents the information for a mechanical mechanism or closure that can cover."@en .

:Electric a owl:Class ;
	rdfs:subClassOf :Systems ;
	rdfs:comment "electric is an XML container that represents the information for the main power supply for device piece of equipment and the distribution of that power throughout the equipment. "@en .

:Enclosure a owl:Class ;
	rdfs:subClassOf :Systems ;
	rdfs:comment "enclosure is an XML container that represents the information for a structure used to contain or isolate a piece of equipment or area."@en .

:EndEffector a owl:Class ;
	rdfs:subClassOf :Component ;
	rdfs:comment "endeffector is an XML container that represents the information for those functions that form the last link segment of a robot. It is the part of the robot that interacts with the manufacturing process."@en .

:Environmental a owl:Class ;
	rdfs:subClassOf :Auxiliaries ;
	rdfs:comment "environmental is an XML container that represents the information for a unit or function involved in monitoring, managing, or conditioning the environment around or within a piece of equipment."@en .

:Feeder a owl:Class ;
	rdfs:subClassOf :Systems ;
	rdfs:comment "feeder is an XML container that represents the information for a system that manages the delivery of materials within a piece of equipment. "@en .

:Hydraulic a owl:Class ;
	rdfs:subClassOf :Systems ;
	rdfs:comment "hydraulic is an XML container that represents the information for a system comprised of all the parts involved in moving and distributing pressurized liquid throughout the piece of equipment."@en .

:Interface a owl:Class ;
	rdfs:subClassOf :Component ;
	rdfs:comment "Each interface component contains data entity available from the piece of equipment that may be needed to coordinate activities with associated pieces of equipment."@en .

:Interfaces a owl:Class ;
	rdfs:subClassOf :Component ;
	rdfs:comment "An XML container that organizes information used to coordinate actions and activities between pieces of equipment that communicate information between each other. "@en .

:Linear a owl:Class ;
	rdfs:subClassOf :Axes ;
	rdfs:comment "A linear axis represents the movement of a physical piece of equipment, or a portion of the equipment, in a straight line. "@en .

:Loader a owl:Class ;
	rdfs:subClassOf :Auxiliaries ;
	rdfs:comment "loader is an XML container that represents the information for a unit comprised of all the parts involved in moving and distributing materials, parts, tooling, and other items to or from a piece of equipment."@en .

:Lubrication a owl:Class ;
	rdfs:subClassOf :Systems ;
	rdfs:comment "lubrication is an XML container that represents the information for a system comprised of all the parts involved in distribution and management of fluids used to lubricate portions of the piece of equipment."@en .

:Materials a owl:Class ;
	rdfs:subClassOf :Resources ;
	rdfs:comment "materials is an XML container that provides information about materials or other items consumed or used by the piece of equipment for production of parts, materials, or other types of goods."@en .

:Path a owl:Class ;
	rdfs:subClassOf :Controller ;
	rdfs:comment "path is an XML container that represents the information for an independent operation or function within a controller."@en .

:Personnel a owl:Class ;
	rdfs:subClassOf :Resources ;
	rdfs:comment "personnel is an XML container that provides information about an individual or individuals who either control, support, or otherwise interface with a piece of equipment."@en .

:Pneumatic a owl:Class ;
	rdfs:subClassOf :Systems ;
	rdfs:comment "pneumatic is an XML container that represents the information for a system comprised of all the parts involved in moving and distributing pressurized gas throughout the piece of equipment."@en .

:Power a owl:Class ;
	rdfs:subClassOf :Component ;
	rdfs:comment "DEPRECATED: power was DEPRECATED in MTConnect Version 1.1 and was replaced by the data entity called availability event."@en .

:ProcessPower a owl:Class ;
	rdfs:subClassOf :Systems ;
	rdfs:comment "processpower is an XML container that represents the information for a power source associated with a piece of equipment that supplies energy to the manufacturing process separate from the electric system."@en .

:Protective a owl:Class ;
	rdfs:subClassOf :Systems ;
	rdfs:comment "Protective is an XML container that represents the information for those functions that detect or prevent harm or damage to equipment or personnel."@en .

:Resources a owl:Class ;
	rdfs:subClassOf :Component ;
	rdfs:comment "An XML container used to organize information for lower level elements representing types of items, materials, and personnel that support the operation of a piece of equipment or work to be performed at a location. resources also represents materials or other items consumed or transformed by a piece of equipment for production of parts or other types of goods."@en .

:Rotary a owl:Class ;
	rdfs:subClassOf :Axes ;
	rdfs:comment "A rotary axis represents any non-linear or rotary movement of a physical piece of equipment or a portion of the equipment. "@en .

:Sensor a owl:Class ;
	rdfs:subClassOf :Auxiliaries ;
	rdfs:comment "The sensor unit is modeled as a lower level component called sensor."@en .

:Stock a owl:Class ;
	rdfs:subClassOf :Materials ;
	rdfs:comment "stock is an XML container that represents the information for the material that is used in a manufacturing process and to which work is applied in a machine or piece of equipment to produce parts."@en .

:Systems a owl:Class ;
	rdfs:subClassOf :Component ;
	rdfs:comment "An XML container used to organize information for lower level elements representing the major sub-systems that are permanently integrated into a piece of equipment."@en .

:ToolingDelivery a owl:Class ;
	rdfs:subClassOf :Auxiliaries ;
	rdfs:comment "toolingdelivery is an XML container that represents the information for a unit involved in managing, positioning, storing, and delivering tooling within a piece of equipment."@en .

:WasteDisposal a owl:Class ;
	rdfs:subClassOf :Auxiliaries ;
	rdfs:comment "wastedisposal is an XML container that represents the information for a unit comprised of all the parts involved in removing manufacturing byproducts from a piece of equipment."@en .

:LeafComponent a owl:Class ;
	rdfs:subClassOf :Component ;
	rdfs:comment "Leaf components are referred to as Composition elements in the MTConnect Standard"@en .

:Actuator a owl:Class ;
	rdfs:subClassOf :LeafComponent ;
	rdfs:comment "A mechanism for moving or controlling a mechanical part of a piece of equipment.    It takes energy usually provided by air, electric current, or liquid and converts the energy into some kind of motion. "@en .

:Amplifier a owl:Class ;
	rdfs:subClassOf :LeafComponent ;
	rdfs:comment "An electronic component or circuit for amplifying power, electric current, or voltage."@en .

:Ballscrew a owl:Class ;
	rdfs:subClassOf :LeafComponent ;
	rdfs:comment "A mechanical structure for transforming rotary motion into linear motion."@en .

:Belt a owl:Class ;
	rdfs:subClassOf :LeafComponent ;
	rdfs:comment "An endless flexible band used to transmit motion for a piece of equipment or to convey materials and objects."@en .

:Brake a owl:Class ;
	rdfs:subClassOf :LeafComponent ;
	rdfs:comment "A mechanism for slowing or stopping a moving object by the absorption or transfer of the energy of momentum, usually by means of friction, electrical force, or magnetic force."@en .

:Chain a owl:Class ;
	rdfs:subClassOf :LeafComponent ;
	rdfs:comment "An interconnected series of objects that band together and are used to transmit motion for a piece of equipment or to convey materials and objects."@en .

:Chopper a owl:Class ;
	rdfs:subClassOf :LeafComponent ;
	rdfs:comment "A mechanism used to break material into smaller pieces."@en .

:Chuck a owl:Class ;
	rdfs:subClassOf :LeafComponent ;
	rdfs:comment "A mechanism that holds a part, stock material, or any other item in place."@en .

:Chute a owl:Class ;
	rdfs:subClassOf :LeafComponent ;
	rdfs:comment "An inclined channel for conveying material."@en .

:CircuitBreaker a owl:Class ;
	rdfs:subClassOf :LeafComponent ;
	rdfs:comment "A mechanism for interrupting an electric circuit."@en .

:Clamp a owl:Class ;
	rdfs:subClassOf :LeafComponent ;
	rdfs:comment "A mechanism used to strengthen, support, or fasten objects in place."@en .

:Compressor a owl:Class ;
	rdfs:subClassOf :LeafComponent ;
	rdfs:comment "A pump or other mechanism for reducing volume and increasing pressure of gases in order to condense the gases to drive pneumatically powered pieces of equipment."@en .

:Door a owl:Class ;
	rdfs:subClassOf :LeafComponent ;
	rdfs:comment "A mechanical mechanism or closure that can cover a physical access portal into a piece of equipment allowing or restricting access to other parts of the equipment."@en .

:Drain a owl:Class ;
	rdfs:subClassOf :LeafComponent ;
	rdfs:comment "A mechanism that allows material to flow for the purpose of drainage from, for example, a vessel or tank."@en .

:Encoder a owl:Class ;
	rdfs:subClassOf :LeafComponent ;
	rdfs:comment "A mechanism used to measure rotary position."@en .

:ExposureUnit a owl:Class ;
	rdfs:subClassOf :LeafComponent ;
	rdfs:comment "A mechanism for emitting a type of radiation"@en .

:ExtrusionUnit a owl:Class ;
	rdfs:subClassOf :LeafComponent ;
	rdfs:comment "A mechanism for dispensing liquid or powered materials"@en .

:Fan a owl:Class ;
	rdfs:subClassOf :LeafComponent ;
	rdfs:comment "Any mechanism for producing a current of air."@en .

:Filter a owl:Class ;
	rdfs:subClassOf :LeafComponent ;
	rdfs:comment "Any substance or structure through which liquids or gases are passed to remove suspended impurities or to recover solids."@en .

:Galvanomotor a owl:Class ;
	rdfs:subClassOf :LeafComponent ;
	rdfs:comment "An electromechanical actuator that produces deflection of a beam of light or energy in response to electric current through its coil in a magnetic field."@en .

:Gripper a owl:Class ;
	rdfs:subClassOf :LeafComponent ;
	rdfs:comment "A mechanism that holds a part, stock material, or any other item in place."@en .

:Hopper a owl:Class ;
	rdfs:subClassOf :LeafComponent ;
	rdfs:comment "A chamber or bin in which materials are stored temporarily, typically being filled through the top and dispensed through the bottom."@en .

:LinearPositionFeedback a owl:Class ;
	rdfs:subClassOf :LeafComponent ;
	rdfs:comment "A mechanism that measures linear motion or position."@en .

:Motor a owl:Class ;
	rdfs:subClassOf :LeafComponent ;
	rdfs:comment "A mechanism that converts electrical, pneumatic, or hydraulic energy into mechanical energy."@en .

:Oil a owl:Class ;
	rdfs:subClassOf :LeafComponent ;
	rdfs:comment "A viscous liquid."@en .

:PowerSupply a owl:Class ;
	rdfs:subClassOf :LeafComponent ;
	rdfs:comment "A unit that provides power to electric mechanisms."@en .

:Pulley a owl:Class ;
	rdfs:subClassOf :LeafComponent ;
	rdfs:comment "A mechanism or wheel that turns in a frame or block and serves to change the direction of or to transmit force."@en .

:Pump a owl:Class ;
	rdfs:subClassOf :LeafComponent ;
	rdfs:comment "An apparatus raising, driving, exhausting, or compressing fluids or gases by means of a piston, plunger, or set of rotating vanes."@en .

:Reel a owl:Class ;
	rdfs:subClassOf :LeafComponent ;
	rdfs:comment "A rotary storage unit for material"@en .

:SensingElement a owl:Class ;
	rdfs:subClassOf :LeafComponent ;
	rdfs:comment "A mechanism that provides a signal or measured value."@en .

:Spreader a owl:Class ;
	rdfs:subClassOf :LeafComponent ;
	rdfs:comment "A mechanism for flattening or spreading materials"@en .

:StorageBattery a owl:Class ;
	rdfs:subClassOf :LeafComponent ;
	rdfs:comment "A component consisting of one or more cells, in which chemical energy is converted into electricity and used as a source of power. "@en .

:Switch a owl:Class ;
	rdfs:subClassOf :LeafComponent ;
	rdfs:comment "A mechanism for turning on or off an electric current or for making or breaking a circuit."@en .

:Table a owl:Class ;
	rdfs:subClassOf :LeafComponent ;
	rdfs:comment "A surface for holding an object or material"@en .

:Tank a owl:Class ;
	rdfs:subClassOf :LeafComponent ;
	rdfs:comment "A receptacle or container for holding material."@en .

:Tensioner a owl:Class ;
	rdfs:subClassOf :LeafComponent ;
	rdfs:comment "A mechanism that provides or applies a stretch or strain to another mechanism."@en .

:Transformer a owl:Class ;
	rdfs:subClassOf :LeafComponent ;
	rdfs:comment "A mechanism that transforms electric energy from a source to a secondary circuit."@en .

:Valve a owl:Class ;
	rdfs:subClassOf :LeafComponent ;
	rdfs:comment "Any mechanism for halting or controlling the flow of a liquid, gas, or other material through a passage, pipe, inlet, or outlet."@en .

:Vat a owl:Class ;
	rdfs:subClassOf :LeafComponent ;
	rdfs:comment "A container for liquid or powdered materials"@en .

:Water a owl:Class ;
	rdfs:subClassOf :LeafComponent ;
	rdfs:comment "A fluid."@en .

:Wire a owl:Class ;
	rdfs:subClassOf :LeafComponent ;
	rdfs:comment "A string like piece or filament of relatively rigid or flexible material provided in a variety of diameters."@en .

[ rdf:type owl:AllDisjointClasses ;
        owl:members (
           :Actuator
           :Auxiliaries
           :Axes
           :Controller
           :Deposition
           :Door
           :EndEffector
           :Interface
           :Interfaces
           :Power
           :Resources
           :Systems
            )
        ] .

[ rdf:type owl:AllDisjointClasses ;
        owl:members (
           :BarFeeder
           :Environmental
           :Loader
           :Sensor
           :ToolingDelivery
           :WasteDisposal
            )
        ] .

[ rdf:type owl:AllDisjointClasses ;
        owl:members (
           :Coolant
           :Dielectric
           :Electric
           :Enclosure
           :Feeder
           :Hydraulic
           :Lubrication
           :Pneumatic
           :ProcessPower
           :Protective
            )
        ] .

[ rdf:type owl:AllDisjointClasses ;
        owl:members (
           :Linear
           :Rotary
            )
        ] .

[ rdf:type owl:AllDisjointClasses ;
        owl:members (
           :Materials
           :Personnel
            )
        ] .

[ rdf:type owl:AllDisjointClasses ;
        owl:members (
           :Actuator
           :Amplifier
           :Ballscrew
           :Belt
           :Brake
           :Chain
           :Chopper
           :Chuck
           :Chute
           :CircuitBreaker
           :Clamp
           :Compressor
           :Door
           :Drain
           :Encoder
           :ExposureUnit
           :ExtrusionUnit
           :Fan
           :Filter
           :Galvanomotor
           :Gripper
           :Hopper
           :LinearPositionFeedback
           :Motor
           :Oil
           :PowerSupply
           :Pulley
           :Pump
           :Reel
           :SensingElement
           :Spreader
           :StorageBattery
           :Switch
           :Table
           :Tank
           :Tensioner
           :Transformer
           :Valve
           :Vat
           :Water
           :Wire
            )
        ] .

:ActiveAxes a owl:Class ;
	rdfs:subClassOf :Event ;
	rdfs:comment "The set of axes currently associated with a path or controller structural element."@en .

:hasActiveAxesValue a owl:DatatypeProperty ;
	rdfs:subPropertyOf :hasEventValue ;
        rdfs:range xsd:string ;
	rdfs:comment "Observed result for: The set of axes currently associated with a path or controller structural element."@en .

:ActuatorState a owl:Class ;
    owl:equivalentClass [ owl:intersectionOf ( :State 
            [ rdf:type owl:Class ;
                owl:oneOf (
                    :ACTIVE
                    :INACTIVE
                    )
                ]
            ) ;
            a owl:Class
        ] .

:hasActuatorState a owl:ObjectProperty ;
	rdfs:subPropertyOf :hasState ;
        rdfs:range :ActuatorState ;
	rdfs:comment "Observed result for: Represents the operational state of an apparatus for moving or controlling a mechanism or system."@en .

:Alarm a owl:Class ;
	rdfs:subClassOf :Event ;
	rdfs:comment "DEPRECATED: Replaced with condition category category data items in Version 1.1.0."@en .

:hasAlarmValue a owl:DatatypeProperty ;
	rdfs:subPropertyOf :hasEventValue ;
        rdfs:range xsd:string ;
	rdfs:comment "Observed result for: DEPRECATED: Replaced with condition category category data items in Version 1.1.0."@en .

:AssetChanged a owl:Class ;
	rdfs:subClassOf :Event ;
	rdfs:comment "The value of the cdata for the event MUST be the assetid of the asset that has been added or changed. There will not be a separate message for new assets."@en .

:hasAssetChangedValue a owl:DatatypeProperty ;
	rdfs:subPropertyOf :hasEventValue ;
        rdfs:range xsd:string ;
	rdfs:comment "Observed result for: The value of the cdata for the event MUST be the assetid of the asset that has been added or changed. There will not be a separate message for new assets."@en .

:AssetRemoved a owl:Class ;
	rdfs:subClassOf :Event ;
	rdfs:comment "The value of the cdata for the event MUST be the assetid of the asset that has been removed. The asset will still be visible if requested with the includeremoved parameter as described in the protocol section. When assets are removed they are not moved to the beginning of the most recently modified list. "@en .

:hasAssetRemovedValue a owl:DatatypeProperty ;
	rdfs:subPropertyOf :hasEventValue ;
        rdfs:range xsd:string ;
	rdfs:comment "Observed result for: The value of the cdata for the event MUST be the assetid of the asset that has been removed. The asset will still be visible if requested with the includeremoved parameter as described in the protocol section. When assets are removed they are not moved to the beginning of the most recently modified list. "@en .

:Availability a owl:Class ;
    owl:equivalentClass [ owl:intersectionOf ( :State 
            [ rdf:type owl:Class ;
                owl:oneOf (
                    :AVAILABLE
                    :UNAVAILABLE
                    )
                ]
            ) ;
            a owl:Class
        ] .

:hasAvailability a owl:ObjectProperty ;
	rdfs:subPropertyOf :hasState ;
        rdfs:range :Availability ;
	rdfs:comment "Observed result for: Represents the agent's ability to communicate with the data source."@en .

:AxisCoupling a owl:Class ;
    owl:equivalentClass [ owl:intersectionOf ( :State 
            [ rdf:type owl:Class ;
                owl:oneOf (
                    :TANDEM
                    :SYNCHRONOUS
                    :MASTER
                    :SLAVE
                    )
                ]
            ) ;
            a owl:Class
        ] .

:hasAxisCoupling a owl:ObjectProperty ;
	rdfs:subPropertyOf :hasState ;
        rdfs:range :AxisCoupling ;
	rdfs:comment "Observed result for: Describes the way the axes will be associated to each other.    This is used in conjunction with coupledaxes event to indicate the way they are interacting."@en .

:AxisFeedrateOverride a owl:Class ;
	rdfs:subClassOf :Event ;
	rdfs:comment "The value of a signal or calculation issued to adjust the feedrate of an individual linear type axis."@en .

:hasAxisFeedrateOverrideValue a owl:DatatypeProperty ;
	rdfs:subPropertyOf :hasEventValue ;
        rdfs:range xsd:string ;
	rdfs:comment "Observed result for: The value of a signal or calculation issued to adjust the feedrate of an individual linear type axis."@en .

:JogAxisFeedrateOverride a owl:Class ;
	rdfs:subClassOf :AxisFeedrateOverride ;
	rdfs:comment "The feedrate specified by a logic or motion program, by a pre-set value, or set by a switch as the feedrate for the axes. "@en .

:hasJogAxisFeedrateOverrideValue a owl:DatatypeProperty ;
	rdfs:subPropertyOf :hasAxisFeedrateOverrideValue ;
        rdfs:range xsd:string ;
	rdfs:comment "Observed result for: The feedrate specified by a logic or motion program, by a pre-set value, or set by a switch as the feedrate for the axes. "@en .

:ProgrammedAxisFeedrateOverride a owl:Class ;
	rdfs:subClassOf :AxisFeedrateOverride ;
	rdfs:comment "The value of a signal or calculation specified by a logic or motion program or set by a switch."@en .

:hasProgrammedAxisFeedrateOverrideValue a owl:DatatypeProperty ;
	rdfs:subPropertyOf :hasAxisFeedrateOverrideValue ;
        rdfs:range xsd:string ;
	rdfs:comment "Observed result for: The value of a signal or calculation specified by a logic or motion program or set by a switch."@en .

:RapidAxisFeedrateOverride a owl:Class ;
	rdfs:subClassOf :AxisFeedrateOverride ;
	rdfs:comment "The value of a signal or calculation issued to adjust the feedrate of a component or composition that is operating in a rapid positioning mode."@en .

:hasRapidAxisFeedrateOverrideValue a owl:DatatypeProperty ;
	rdfs:subPropertyOf :hasAxisFeedrateOverrideValue ;
        rdfs:range xsd:string ;
	rdfs:comment "Observed result for: The value of a signal or calculation issued to adjust the feedrate of a component or composition that is operating in a rapid positioning mode."@en .

[ rdf:type owl:AllDisjointClasses ;
        owl:members (
           :JogAxisFeedrateOverride
           :ProgrammedAxisFeedrateOverride
           :RapidAxisFeedrateOverride
            )
        ] .

:AxisInterlock a owl:Class ;
    owl:equivalentClass [ owl:intersectionOf ( :State 
            [ rdf:type owl:Class ;
                owl:oneOf (
                    :ACTIVE
                    :INACTIVE
                    )
                ]
            ) ;
            a owl:Class
        ] .

:hasAxisInterlock a owl:ObjectProperty ;
	rdfs:subPropertyOf :hasState ;
        rdfs:range :AxisInterlock ;
	rdfs:comment "Observed result for: An indicator of the state of the axis lockout function when power has been removed and the axis is allowed to move freely."@en .

:AxisState a owl:Class ;
    owl:equivalentClass [ owl:intersectionOf ( :State 
            [ rdf:type owl:Class ;
                owl:oneOf (
                    :HOME
                    :TRAVEL
                    :PARKED
                    :STOPPED
                    )
                ]
            ) ;
            a owl:Class
        ] .

:hasAxisState a owl:ObjectProperty ;
	rdfs:subPropertyOf :hasState ;
        rdfs:range :AxisState ;
	rdfs:comment "Observed result for: An indicator of the controlled state of a linear or rotary component representing an axis."@en .

:Block a owl:Class ;
	rdfs:subClassOf :Event ;
	rdfs:comment "The line of code or command being executed by a controller structural element."@en .

:hasBlockValue a owl:DatatypeProperty ;
	rdfs:subPropertyOf :hasEventValue ;
        rdfs:range xsd:string ;
	rdfs:comment "Observed result for: The line of code or command being executed by a controller structural element."@en .

:BlockCount a owl:Class ;
	rdfs:subClassOf :Event ;
	rdfs:comment "The total count of the number of blocks of program code that have been executed since execution started."@en .

:hasBlockCountValue a owl:DatatypeProperty ;
	rdfs:subPropertyOf :hasEventValue ;
        rdfs:range xsd:string ;
	rdfs:comment "Observed result for: The total count of the number of blocks of program code that have been executed since execution started."@en .

:ChuckInterlock a owl:Class ;
    owl:equivalentClass [ owl:intersectionOf ( :State 
            [ rdf:type owl:Class ;
                owl:oneOf (
                    :ACTIVE
                    :INACTIVE
                    )
                ]
            ) ;
            a owl:Class
        ] .

:hasChuckInterlock a owl:ObjectProperty ;
	rdfs:subPropertyOf :hasState ;
        rdfs:range :ChuckInterlock ;
	rdfs:comment "Observed result for: An indication of the state of an interlock function or control logic state intended to prevent the associated chuck component from being operated."@en .

:ManualUnclampChuckInterlock a owl:Class ;
	rdfs:subClassOf :ChuckInterlock ;
	rdfs:comment "An indication of the state of an operator controlled interlock that can inhibit the ability to initiate an unclamp action of an electronically controlled chuck. The valid data value must be active value or inactive value.  When manualunclamp subtype is active value, it is expected that a chuck cannot be unclamped until manualunclamp subtype is set to inactive value. "@en .

:hasManualUnclampChuckInterlock a owl:ObjectProperty ;
	rdfs:subPropertyOf :hasChuckInterlock ;
        rdfs:range :ChuckInterlock ;
	rdfs:comment "Observed result for: An indication of the state of an operator controlled interlock that can inhibit the ability to initiate an unclamp action of an electronically controlled chuck. The valid data value must be active value or inactive value.  When manualunclamp subtype is active value, it is expected that a chuck cannot be unclamped until manualunclamp subtype is set to inactive value. "@en .

:ChuckState a owl:Class ;
    owl:equivalentClass [ owl:intersectionOf ( :State 
            [ rdf:type owl:Class ;
                owl:oneOf (
                    :OPEN
                    :CLOSED
                    :UNLATCHED
                    )
                ]
            ) ;
            a owl:Class
        ] .

:hasChuckState a owl:ObjectProperty ;
	rdfs:subPropertyOf :hasState ;
        rdfs:range :ChuckState ;
	rdfs:comment "Observed result for: An indication of the operating state of a mechanism that holds a part or stock material during a manufacturing process. It may also represent a mechanism that holds any other mechanism in place within a piece of equipment."@en .

:CloseChuck a owl:Class ;
	rdfs:subClassOf :Event ;
	rdfs:comment "Service to close a chuck."@en .

:hasCloseChuckValue a owl:DatatypeProperty ;
	rdfs:subPropertyOf :hasEventValue ;
        rdfs:range xsd:string ;
	rdfs:comment "Observed result for: Service to close a chuck."@en .

:CloseDoor a owl:Class ;
	rdfs:subClassOf :Event ;
	rdfs:comment "Service to close a door."@en .

:hasCloseDoorValue a owl:DatatypeProperty ;
	rdfs:subPropertyOf :hasEventValue ;
        rdfs:range xsd:string ;
	rdfs:comment "Observed result for: Service to close a door."@en .

:Code a owl:Class ;
	rdfs:subClassOf :Event ;
	rdfs:comment "DEPRECATED in Version 1.1."@en .

:hasCodeValue a owl:DatatypeProperty ;
	rdfs:subPropertyOf :hasEventValue ;
        rdfs:range xsd:string ;
	rdfs:comment "Observed result for: DEPRECATED in Version 1.1."@en .

:CompositionState a owl:Class ;
	rdfs:subClassOf :Event ;
	rdfs:comment "An indication of the operating condition of a mechanism represented by a composition type element."@en .

:hasCompositionStateValue a owl:DatatypeProperty ;
	rdfs:subPropertyOf :hasEventValue ;
        rdfs:range xsd:string ;
	rdfs:comment "Observed result for: An indication of the operating condition of a mechanism represented by a composition type element."@en .

:ActionCompositionState a owl:Class ;
	rdfs:subClassOf :CompositionState ;
	rdfs:comment "An indication of the operating state of a mechanism represented by a composition type component. The operating state indicates whether the composition element is activated or disabled.  The valid data value must be active value or inactive value."@en .

:hasActionCompositionStateValue a owl:DatatypeProperty ;
	rdfs:subPropertyOf :hasCompositionStateValue ;
        rdfs:range xsd:string ;
	rdfs:comment "Observed result for: An indication of the operating state of a mechanism represented by a composition type component. The operating state indicates whether the composition element is activated or disabled.  The valid data value must be active value or inactive value."@en .

:LateralCompositionState a owl:Class ;
	rdfs:subClassOf :CompositionState ;
	rdfs:comment "An indication of the position of a mechanism that may move in a lateral direction.   The mechanism is represented by a composition type component.  The position information indicates whether the composition element is positioned to the right, to the left, or is in transition.   The valid data value must be right value, left value, or transitioning value."@en .

:hasLateralCompositionStateValue a owl:DatatypeProperty ;
	rdfs:subPropertyOf :hasCompositionStateValue ;
        rdfs:range xsd:string ;
	rdfs:comment "Observed result for: An indication of the position of a mechanism that may move in a lateral direction.   The mechanism is represented by a composition type component.  The position information indicates whether the composition element is positioned to the right, to the left, or is in transition.   The valid data value must be right value, left value, or transitioning value."@en .

:MotionCompositionState a owl:Class ;
	rdfs:subClassOf :CompositionState ;
	rdfs:comment "An indication of the open or closed state of a mechanism.   The mechanism is represented by a composition type component.  The operating state indicates whether the state of the composition element is open, closed, or unlatched.    The valid data value must be open value, unlatched value, or closed value."@en .

:hasMotionCompositionStateValue a owl:DatatypeProperty ;
	rdfs:subPropertyOf :hasCompositionStateValue ;
        rdfs:range xsd:string ;
	rdfs:comment "Observed result for: An indication of the open or closed state of a mechanism.   The mechanism is represented by a composition type component.  The operating state indicates whether the state of the composition element is open, closed, or unlatched.    The valid data value must be open value, unlatched value, or closed value."@en .

:SwitchedCompositionState a owl:Class ;
	rdfs:subClassOf :CompositionState ;
	rdfs:comment "An indication of the activation state of a mechanism represented by a composition type component. The activation state indicates whether the composition element is activated or not. The valid data value must be on value or off value."@en .

:hasSwitchedCompositionStateValue a owl:DatatypeProperty ;
	rdfs:subPropertyOf :hasCompositionStateValue ;
        rdfs:range xsd:string ;
	rdfs:comment "Observed result for: An indication of the activation state of a mechanism represented by a composition type component. The activation state indicates whether the composition element is activated or not. The valid data value must be on value or off value."@en .

:VerticalCompositionState a owl:Class ;
	rdfs:subClassOf :CompositionState ;
	rdfs:comment "An indication of the position of a mechanism that may move in a vertical direction. The mechanism is represented by a composition type component.  The position information indicates whether the composition element is positioned to the top, to the bottom, or is in transition.   The valid data value must be up value, down value, or transitioning value."@en .

:hasVerticalCompositionStateValue a owl:DatatypeProperty ;
	rdfs:subPropertyOf :hasCompositionStateValue ;
        rdfs:range xsd:string ;
	rdfs:comment "Observed result for: An indication of the position of a mechanism that may move in a vertical direction. The mechanism is represented by a composition type component.  The position information indicates whether the composition element is positioned to the top, to the bottom, or is in transition.   The valid data value must be up value, down value, or transitioning value."@en .

[ rdf:type owl:AllDisjointClasses ;
        owl:members (
           :ActionCompositionState
           :LateralCompositionState
           :MotionCompositionState
           :SwitchedCompositionState
           :VerticalCompositionState
            )
        ] .

:ControllerMode a owl:Class ;
    owl:equivalentClass [ owl:intersectionOf ( :State 
            [ rdf:type owl:Class ;
                owl:oneOf (
                    :AUTOMATIC
                    :MANUAL
                    :MANUAL_DATA_INPUT
                    :SEMI_AUTOMATIC
                    :EDIT
                    )
                ]
            ) ;
            a owl:Class
        ] .

:hasControllerMode a owl:ObjectProperty ;
	rdfs:subPropertyOf :hasState ;
        rdfs:range :ControllerMode ;
	rdfs:comment "Observed result for: The current operating mode of the controller component."@en .

:ControllerModeOverride a owl:Class ;
    owl:equivalentClass [ owl:intersectionOf ( :State 
            [ rdf:type owl:Class ;
                owl:oneOf (
                    :ON
                    :OFF
                    )
                ]
            ) ;
            a owl:Class
        ] .

:hasControllerModeOverride a owl:ObjectProperty ;
	rdfs:subPropertyOf :hasState ;
        rdfs:range :ControllerModeOverride ;
	rdfs:comment "Observed result for: A setting or operator selection that changes the behavior of a piece of equipment."@en .

:DryRunControllerModeOverride a owl:Class ;
	rdfs:subClassOf :ControllerModeOverride ;
	rdfs:comment "A setting or operator selection used to execute a test mode to confirm the execution of machine functions.  The valid data value must be on value or off value.  When dryrun subtype is on value, the equipment performs all of its normal functions, except no part or product is produced.  If the equipment has a spindle, spindle operation is suspended."@en .

:hasDryRunControllerModeOverride a owl:ObjectProperty ;
	rdfs:subPropertyOf :hasControllerModeOverride ;
        rdfs:range :ControllerModeOverride ;
	rdfs:comment "Observed result for: A setting or operator selection used to execute a test mode to confirm the execution of machine functions.  The valid data value must be on value or off value.  When dryrun subtype is on value, the equipment performs all of its normal functions, except no part or product is produced.  If the equipment has a spindle, spindle operation is suspended."@en .

:SingleBlockControllerModeOverride a owl:Class ;
	rdfs:subClassOf :ControllerModeOverride ;
	rdfs:comment "A setting or operator selection that changes the behavior of the controller on a piece of equipment.  The valid data value must be on value or off value. Program execution is paused after each block event of code is executed when singleblock subtype is on value.    When singleblock subtype is on value, execution event must change to interrupted value after completion of each block event of code. "@en .

:hasSingleBlockControllerModeOverride a owl:ObjectProperty ;
	rdfs:subPropertyOf :hasControllerModeOverride ;
        rdfs:range :ControllerModeOverride ;
	rdfs:comment "Observed result for: A setting or operator selection that changes the behavior of the controller on a piece of equipment.  The valid data value must be on value or off value. Program execution is paused after each block event of code is executed when singleblock subtype is on value.    When singleblock subtype is on value, execution event must change to interrupted value after completion of each block event of code. "@en .

:MachineAxisLockControllerModeOverride a owl:Class ;
	rdfs:subClassOf :ControllerModeOverride ;
	rdfs:comment "A setting or operator selection that changes the behavior of the controller on a piece of equipment.  The valid data value must be on value or off value.  When machineaxislock subtype is on value, program execution continues normally, but no equipment motion occurs "@en .

:hasMachineAxisLockControllerModeOverride a owl:ObjectProperty ;
	rdfs:subPropertyOf :hasControllerModeOverride ;
        rdfs:range :ControllerModeOverride ;
	rdfs:comment "Observed result for: A setting or operator selection that changes the behavior of the controller on a piece of equipment.  The valid data value must be on value or off value.  When machineaxislock subtype is on value, program execution continues normally, but no equipment motion occurs "@en .

:OptionalStopControllerModeOverride a owl:Class ;
	rdfs:subClassOf :ControllerModeOverride ;
	rdfs:comment "A setting or operator selection that changes the behavior of the controller on a piece of equipment.  The valid data value must be on value or off value. The program execution is stopped after a specific program block is executed when optionalstop subtype is on value.     In the case of a G-Code program, a program block event containing a M01 code designates the command for an optionalstop subtype.  execution event must change to optionalstop subtype after a program block specifying an optional stop is executed and the optionalstop subtype selection is on value."@en .

:hasOptionalStopControllerModeOverride a owl:ObjectProperty ;
	rdfs:subPropertyOf :hasControllerModeOverride ;
        rdfs:range :ControllerModeOverride ;
	rdfs:comment "Observed result for: A setting or operator selection that changes the behavior of the controller on a piece of equipment.  The valid data value must be on value or off value. The program execution is stopped after a specific program block is executed when optionalstop subtype is on value.     In the case of a G-Code program, a program block event containing a M01 code designates the command for an optionalstop subtype.  execution event must change to optionalstop subtype after a program block specifying an optional stop is executed and the optionalstop subtype selection is on value."@en .

:ToolChangeStopControllerModeOverride a owl:Class ;
	rdfs:subClassOf :ControllerModeOverride ;
	rdfs:comment "A setting or operator selection that changes the behavior of the controller on a piece of equipment.  The valid data value must be on value or off value.  Program execution is paused when a command is executed requesting a cutting tool to be changed.  execution event must change to interrupted value after completion of the command requesting a cutting tool to be changed and toolchangestop subtype is on value."@en .

:hasToolChangeStopControllerModeOverride a owl:ObjectProperty ;
	rdfs:subPropertyOf :hasControllerModeOverride ;
        rdfs:range :ControllerModeOverride ;
	rdfs:comment "Observed result for: A setting or operator selection that changes the behavior of the controller on a piece of equipment.  The valid data value must be on value or off value.  Program execution is paused when a command is executed requesting a cutting tool to be changed.  execution event must change to interrupted value after completion of the command requesting a cutting tool to be changed and toolchangestop subtype is on value."@en .

[ rdf:type owl:AllDisjointClasses ;
        owl:members (
           :DryRunControllerModeOverride
           :SingleBlockControllerModeOverride
           :MachineAxisLockControllerModeOverride
           :OptionalStopControllerModeOverride
           :ToolChangeStopControllerModeOverride
            )
        ] .

:CoupledAxes a owl:Class ;
	rdfs:subClassOf :Event ;
	rdfs:comment "Refers to the set of associated axes."@en .

:hasCoupledAxesValue a owl:DatatypeProperty ;
	rdfs:subPropertyOf :hasEventValue ;
        rdfs:range xsd:string ;
	rdfs:comment "Observed result for: Refers to the set of associated axes."@en .

:DateCode a owl:Class ;
	rdfs:subClassOf :Event ;
	rdfs:comment "The time and date code associated with a material or other physical item.   datecode event MUST be reported in ISO 8601 format."@en .

:hasDateCodeValue a owl:DatatypeProperty ;
	rdfs:subPropertyOf :hasEventValue ;
        rdfs:range xsd:string ;
	rdfs:comment "Observed result for: The time and date code associated with a material or other physical item.   datecode event MUST be reported in ISO 8601 format."@en .

:ManufactureDateCode a owl:Class ;
	rdfs:subClassOf :DateCode ;
	rdfs:comment "The time and date code relating to the production of a material or other physical item."@en .

:hasManufactureDateCodeValue a owl:DatatypeProperty ;
	rdfs:subPropertyOf :hasDateCodeValue ;
        rdfs:range xsd:string ;
	rdfs:comment "Observed result for: The time and date code relating to the production of a material or other physical item."@en .

:ExpirationDateCode a owl:Class ;
	rdfs:subClassOf :DateCode ;
	rdfs:comment "The time and date code relating to the expiration or end of useful life for a material or other physical item."@en .

:hasExpirationDateCodeValue a owl:DatatypeProperty ;
	rdfs:subPropertyOf :hasDateCodeValue ;
        rdfs:range xsd:string ;
	rdfs:comment "Observed result for: The time and date code relating to the expiration or end of useful life for a material or other physical item."@en .

:FirstUseDateCode a owl:Class ;
	rdfs:subClassOf :DateCode ;
	rdfs:comment "The time and date code relating the first use of a material or other physical item."@en .

:hasFirstUseDateCodeValue a owl:DatatypeProperty ;
	rdfs:subPropertyOf :hasDateCodeValue ;
        rdfs:range xsd:string ;
	rdfs:comment "Observed result for: The time and date code relating the first use of a material or other physical item."@en .

[ rdf:type owl:AllDisjointClasses ;
        owl:members (
           :ManufactureDateCode
           :ExpirationDateCode
           :FirstUseDateCode
            )
        ] .

:DeviceUuid a owl:Class ;
	rdfs:subClassOf :Event ;
	rdfs:comment "The identifier of another piece of equipment that is temporarily associated with a component of this piece of equipment to perform a particular function.   The valid data value MUST be a NMTOKEN XML type."@en .

:hasDeviceUuidValue a owl:DatatypeProperty ;
	rdfs:subPropertyOf :hasEventValue ;
        rdfs:range xsd:string ;
	rdfs:comment "Observed result for: The identifier of another piece of equipment that is temporarily associated with a component of this piece of equipment to perform a particular function.   The valid data value MUST be a NMTOKEN XML type."@en .

:Direction a owl:Class ;
	rdfs:subClassOf :Event ;
	rdfs:comment "The direction of motion."@en .

:hasDirectionValue a owl:DatatypeProperty ;
	rdfs:subPropertyOf :hasEventValue ;
        rdfs:range xsd:string ;
	rdfs:comment "Observed result for: The direction of motion."@en .

:RotaryDirection a owl:Class ;
	rdfs:subClassOf :Direction ;
	rdfs:comment "The rotational direction of a rotary motion using the right hand rule convention. The valid data value must be clockwise value or counterclockwise value."@en .

:hasRotaryDirectionValue a owl:DatatypeProperty ;
	rdfs:subPropertyOf :hasDirectionValue ;
        rdfs:range xsd:string ;
	rdfs:comment "Observed result for: The rotational direction of a rotary motion using the right hand rule convention. The valid data value must be clockwise value or counterclockwise value."@en .

:LinearDirection a owl:Class ;
	rdfs:subClassOf :Direction ;
	rdfs:comment "The direction of motion of a linear motion."@en .

:hasLinearDirectionValue a owl:DatatypeProperty ;
	rdfs:subPropertyOf :hasDirectionValue ;
        rdfs:range xsd:string ;
	rdfs:comment "Observed result for: The direction of motion of a linear motion."@en .

[ rdf:type owl:AllDisjointClasses ;
        owl:members (
           :RotaryDirection
           :LinearDirection
            )
        ] .

:DoorState a owl:Class ;
    owl:equivalentClass [ owl:intersectionOf ( :State 
            [ rdf:type owl:Class ;
                owl:oneOf (
                    :CLOSED
                    :CLOSED
                    :UNLATCHED
                    )
                ]
            ) ;
            a owl:Class
        ] .

:hasDoorState a owl:ObjectProperty ;
	rdfs:subPropertyOf :hasState ;
        rdfs:range :DoorState ;
	rdfs:comment "Observed result for: The operational state of a door type component or composition element."@en .

:EmergencyStop a owl:Class ;
    owl:equivalentClass [ owl:intersectionOf ( :State 
            [ rdf:type owl:Class ;
                owl:oneOf (
                    :ARMED
                    :TRIGGERED
                    )
                ]
            ) ;
            a owl:Class
        ] .

:hasEmergencyStop a owl:ObjectProperty ;
	rdfs:subPropertyOf :hasState ;
        rdfs:range :EmergencyStop ;
	rdfs:comment "Observed result for: The current state of the emergency stop signal for a piece of equipment, controller path, or any other component or subsystem of a piece of equipment."@en .

:EndOfBar a owl:Class ;
    owl:equivalentClass [ owl:intersectionOf ( :State 
            [ rdf:type owl:Class ;
                owl:oneOf (
                    :YES
                    :NO
                    )
                ]
            ) ;
            a owl:Class
        ] .

:hasEndOfBar a owl:ObjectProperty ;
	rdfs:subPropertyOf :hasState ;
        rdfs:range :EndOfBar ;
	rdfs:comment "Observed result for: An indication of whether the end of a piece of bar stock being feed by a bar feeder has been reached."@en .

:PrimaryEndOfBar a owl:Class ;
	rdfs:subClassOf :EndOfBar ;
	rdfs:comment "Specific applications MAY reference one or more locations on a piece of bar stock as the indication for the endofbar event. The main or most important location must be designated as the primary subtype indication for the endofbar event.    If no subtype is specified, primary subtype must be the default endofbar event indication."@en .

:hasPrimaryEndOfBar a owl:ObjectProperty ;
	rdfs:subPropertyOf :hasEndOfBar ;
        rdfs:range :EndOfBar ;
	rdfs:comment "Observed result for: Specific applications MAY reference one or more locations on a piece of bar stock as the indication for the endofbar event. The main or most important location must be designated as the primary subtype indication for the endofbar event.    If no subtype is specified, primary subtype must be the default endofbar event indication."@en .

:AuxiliaryEndOfBar a owl:Class ;
	rdfs:subClassOf :EndOfBar ;
	rdfs:comment "When multiple locations on a piece of bar stock are referenced as the indication for the endofbar event, the additional location(s) must be designated as auxiliary subtype indication(s) for the endofbar event.  "@en .

:hasAuxiliaryEndOfBar a owl:ObjectProperty ;
	rdfs:subPropertyOf :hasEndOfBar ;
        rdfs:range :EndOfBar ;
	rdfs:comment "Observed result for: When multiple locations on a piece of bar stock are referenced as the indication for the endofbar event, the additional location(s) must be designated as auxiliary subtype indication(s) for the endofbar event.  "@en .

[ rdf:type owl:AllDisjointClasses ;
        owl:members (
           :PrimaryEndOfBar
           :AuxiliaryEndOfBar
            )
        ] .

:EquipmentMode a owl:Class ;
    owl:equivalentClass [ owl:intersectionOf ( :State 
            [ rdf:type owl:Class ;
                owl:oneOf (
                    :ON
                    :OFF
                    )
                ]
            ) ;
            a owl:Class
        ] .

:hasEquipmentMode a owl:ObjectProperty ;
	rdfs:subPropertyOf :hasState ;
        rdfs:range :EquipmentMode ;
	rdfs:comment "Observed result for: An indication that a piece of equipment, or a sub-part of a piece of equipment, is performing specific types of activities."@en .

:LoadedEquipmentMode a owl:Class ;
	rdfs:subClassOf :EquipmentMode ;
	rdfs:comment "Subparts of a piece of equipment are under load."@en .

:hasLoadedEquipmentMode a owl:ObjectProperty ;
	rdfs:subPropertyOf :hasEquipmentMode ;
        rdfs:range :EquipmentMode ;
	rdfs:comment "Observed result for: Subparts of a piece of equipment are under load."@en .

:WorkingEquipmentMode a owl:Class ;
	rdfs:subClassOf :EquipmentMode ;
	rdfs:comment "A piece of equipment performing any activity, the equipment is active and performing a function under load or not."@en .

:hasWorkingEquipmentMode a owl:ObjectProperty ;
	rdfs:subPropertyOf :hasEquipmentMode ;
        rdfs:range :EquipmentMode ;
	rdfs:comment "Observed result for: A piece of equipment performing any activity, the equipment is active and performing a function under load or not."@en .

:OperatingEquipmentMode a owl:Class ;
	rdfs:subClassOf :EquipmentMode ;
	rdfs:comment "A piece of equipment are powered or performing any activity."@en .

:hasOperatingEquipmentMode a owl:ObjectProperty ;
	rdfs:subPropertyOf :hasEquipmentMode ;
        rdfs:range :EquipmentMode ;
	rdfs:comment "Observed result for: A piece of equipment are powered or performing any activity."@en .

:PoweredEquipmentMode a owl:Class ;
	rdfs:subClassOf :EquipmentMode ;
	rdfs:comment "Primary  power is  applied  to the  piece  of  equipment and,  as  a minimum, the controller or logic portion of the piece of equipment is powered and functioning or components that are required to remain on are powered."@en .

:hasPoweredEquipmentMode a owl:ObjectProperty ;
	rdfs:subPropertyOf :hasEquipmentMode ;
        rdfs:range :EquipmentMode ;
	rdfs:comment "Observed result for: Primary  power is  applied  to the  piece  of  equipment and,  as  a minimum, the controller or logic portion of the piece of equipment is powered and functioning or components that are required to remain on are powered."@en .

:DelayEquipmentMode a owl:Class ;
	rdfs:subClassOf :EquipmentMode ;
	rdfs:comment "A piece of equipment waiting for an event or an action to occur."@en .

:hasDelayEquipmentMode a owl:ObjectProperty ;
	rdfs:subPropertyOf :hasEquipmentMode ;
        rdfs:range :EquipmentMode ;
	rdfs:comment "Observed result for: A piece of equipment waiting for an event or an action to occur."@en .

[ rdf:type owl:AllDisjointClasses ;
        owl:members (
           :LoadedEquipmentMode
           :WorkingEquipmentMode
           :OperatingEquipmentMode
           :PoweredEquipmentMode
           :DelayEquipmentMode
            )
        ] .

:Execution a owl:Class ;
    owl:equivalentClass [ owl:intersectionOf ( :State 
            [ rdf:type owl:Class ;
                owl:oneOf (
                    :READY
                    :ACTIVE
                    :INTERRUPTED
                    :FEED_HOLD
                    :STOPPED
                    :OPTIONAL_STOP
                    :PROGRAM_STOPPED
                    :PROGRAM_COMPLETED
                    )
                ]
            ) ;
            a owl:Class
        ] .

:hasExecution a owl:ObjectProperty ;
	rdfs:subPropertyOf :hasState ;
        rdfs:range :Execution ;
	rdfs:comment "Observed result for: The execution status of the controller."@en .

:FunctionalMode a owl:Class ;
    owl:equivalentClass [ owl:intersectionOf ( :State 
            [ rdf:type owl:Class ;
                owl:oneOf (
                    :PRODUCTION
                    :SETUP
                    :TEARDOWN
                    :MAINTENANCE
                    :PROCESS_DEVELOPMENT
                    )
                ]
            ) ;
            a owl:Class
        ] .

:hasFunctionalMode a owl:ObjectProperty ;
	rdfs:subPropertyOf :hasState ;
        rdfs:range :FunctionalMode ;
	rdfs:comment "Observed result for: The current intended production status of the device or component."@en .

:Hardness a owl:Class ;
	rdfs:subClassOf :Event ;
	rdfs:comment "The measurement of the hardness of a material."@en .

:hasHardnessValue a owl:DatatypeProperty ;
	rdfs:subPropertyOf :hasEventValue ;
        rdfs:range xsd:string ;
	rdfs:comment "Observed result for: The measurement of the hardness of a material."@en .

:RockwellHardness a owl:Class ;
	rdfs:subClassOf :Hardness ;
	rdfs:comment "A scale to measure the resistance to deformation of a surface."@en .

:hasRockwellHardnessValue a owl:DatatypeProperty ;
	rdfs:subPropertyOf :hasHardnessValue ;
        rdfs:range xsd:string ;
	rdfs:comment "Observed result for: A scale to measure the resistance to deformation of a surface."@en .

:VickersHardness a owl:Class ;
	rdfs:subClassOf :Hardness ;
	rdfs:comment "A scale to measure the resistance to deformation of a surface."@en .

:hasVickersHardnessValue a owl:DatatypeProperty ;
	rdfs:subPropertyOf :hasHardnessValue ;
        rdfs:range xsd:string ;
	rdfs:comment "Observed result for: A scale to measure the resistance to deformation of a surface."@en .

:ShoreHardness a owl:Class ;
	rdfs:subClassOf :Hardness ;
	rdfs:comment "A scale to measure the resistance to deformation of a surface."@en .

:hasShoreHardnessValue a owl:DatatypeProperty ;
	rdfs:subPropertyOf :hasHardnessValue ;
        rdfs:range xsd:string ;
	rdfs:comment "Observed result for: A scale to measure the resistance to deformation of a surface."@en .

:BrinellHardness a owl:Class ;
	rdfs:subClassOf :Hardness ;
	rdfs:comment "A scale to measure the resistance to deformation of a surface."@en .

:hasBrinellHardnessValue a owl:DatatypeProperty ;
	rdfs:subPropertyOf :hasHardnessValue ;
        rdfs:range xsd:string ;
	rdfs:comment "Observed result for: A scale to measure the resistance to deformation of a surface."@en .

:LeebHardness a owl:Class ;
	rdfs:subClassOf :Hardness ;
	rdfs:comment "A scale to measure the elasticity of a surface."@en .

:hasLeebHardnessValue a owl:DatatypeProperty ;
	rdfs:subPropertyOf :hasHardnessValue ;
        rdfs:range xsd:string ;
	rdfs:comment "Observed result for: A scale to measure the elasticity of a surface."@en .

:MohsHardness a owl:Class ;
	rdfs:subClassOf :Hardness ;
	rdfs:comment "A scale to measure the resistance to scratching of a surface."@en .

:hasMohsHardnessValue a owl:DatatypeProperty ;
	rdfs:subPropertyOf :hasHardnessValue ;
        rdfs:range xsd:string ;
	rdfs:comment "Observed result for: A scale to measure the resistance to scratching of a surface."@en .

[ rdf:type owl:AllDisjointClasses ;
        owl:members (
           :RockwellHardness
           :VickersHardness
           :ShoreHardness
           :BrinellHardness
           :LeebHardness
           :MohsHardness
            )
        ] .

:InterfaceState a owl:Class ;
    owl:equivalentClass [ owl:intersectionOf ( :State 
            [ rdf:type owl:Class ;
                owl:oneOf (
                    :ENABLED
                    :DISABLED
                    )
                ]
            ) ;
            a owl:Class
        ] .

:hasInterfaceState a owl:ObjectProperty ;
	rdfs:subPropertyOf :hasState ;
        rdfs:range :InterfaceState ;
	rdfs:comment "Observed result for: An indication of the operational state of an interface component component."@en .

:Line a owl:Class ;
	rdfs:subClassOf :Event ;
	rdfs:comment "DEPRECATED in Version 1.4.0."@en .

:hasLineValue a owl:DatatypeProperty ;
	rdfs:subPropertyOf :hasEventValue ;
        rdfs:range xsd:string ;
	rdfs:comment "Observed result for: DEPRECATED in Version 1.4.0."@en .

:MaximumLine a owl:Class ;
	rdfs:subClassOf :Line ;
	rdfs:comment "Maximum value of a data entity or attribute."@en .

:hasMaximumLineValue a owl:DatatypeProperty ;
	rdfs:subPropertyOf :hasLineValue ;
        rdfs:range xsd:string ;
	rdfs:comment "Observed result for: Maximum value of a data entity or attribute."@en .

:MinimumLine a owl:Class ;
	rdfs:subClassOf :Line ;
	rdfs:comment "The minimum value of a data entity or attribute."@en .

:hasMinimumLineValue a owl:DatatypeProperty ;
	rdfs:subPropertyOf :hasLineValue ;
        rdfs:range xsd:string ;
	rdfs:comment "Observed result for: The minimum value of a data entity or attribute."@en .

[ rdf:type owl:AllDisjointClasses ;
        owl:members (
           :MaximumLine
           :MinimumLine
            )
        ] .

:LineLabel a owl:Class ;
	rdfs:subClassOf :Event ;
	rdfs:comment "An optional identifier for a block event of code in a program event."@en .

:hasLineLabelValue a owl:DatatypeProperty ;
	rdfs:subPropertyOf :hasEventValue ;
        rdfs:range xsd:string ;
	rdfs:comment "Observed result for: An optional identifier for a block event of code in a program event."@en .

:LineNumber a owl:Class ;
	rdfs:subClassOf :Event ;
	rdfs:comment "A reference to the position of a block of program code within a control program."@en .

:hasLineNumberValue a owl:DatatypeProperty ;
	rdfs:subPropertyOf :hasEventValue ;
        rdfs:range xsd:string ;
	rdfs:comment "Observed result for: A reference to the position of a block of program code within a control program."@en .

:AbsoluteLineNumber a owl:Class ;
	rdfs:subClassOf :LineNumber ;
	rdfs:comment "The position of a block of program code relative to the beginning of the control program."@en .

:hasAbsoluteLineNumberValue a owl:DatatypeProperty ;
	rdfs:subPropertyOf :hasLineNumberValue ;
        rdfs:range xsd:string ;
	rdfs:comment "Observed result for: The position of a block of program code relative to the beginning of the control program."@en .

:IncrementalLineNumber a owl:Class ;
	rdfs:subClassOf :LineNumber ;
	rdfs:comment "The position of a block of program code relative to the occurrence of the last linelabel event encountered in the control program."@en .

:hasIncrementalLineNumberValue a owl:DatatypeProperty ;
	rdfs:subPropertyOf :hasLineNumberValue ;
        rdfs:range xsd:string ;
	rdfs:comment "Observed result for: The position of a block of program code relative to the occurrence of the last linelabel event encountered in the control program."@en .

[ rdf:type owl:AllDisjointClasses ;
        owl:members (
           :AbsoluteLineNumber
           :IncrementalLineNumber
            )
        ] .

:Material a owl:Class ;
	rdfs:subClassOf :Event ;
	rdfs:comment "The identifier of a material used or consumed in the manufacturing process."@en .

:hasMaterialValue a owl:DatatypeProperty ;
	rdfs:subPropertyOf :hasEventValue ;
        rdfs:range xsd:string ;
	rdfs:comment "Observed result for: The identifier of a material used or consumed in the manufacturing process."@en .

:MaterialChange a owl:Class ;
	rdfs:subClassOf :Event ;
	rdfs:comment "Service to change the type of material or product being loaded or fed to a piece of equipment."@en .

:hasMaterialChangeValue a owl:DatatypeProperty ;
	rdfs:subPropertyOf :hasEventValue ;
        rdfs:range xsd:string ;
	rdfs:comment "Observed result for: Service to change the type of material or product being loaded or fed to a piece of equipment."@en .

:MaterialFeed a owl:Class ;
	rdfs:subClassOf :Event ;
	rdfs:comment "Service to advance material or feed product to a piece of equipment from a continuous or bulk source. "@en .

:hasMaterialFeedValue a owl:DatatypeProperty ;
	rdfs:subPropertyOf :hasEventValue ;
        rdfs:range xsd:string ;
	rdfs:comment "Observed result for: Service to advance material or feed product to a piece of equipment from a continuous or bulk source. "@en .

:MaterialLayer a owl:Class ;
	rdfs:subClassOf :Event ;
	rdfs:comment "Identifies the layers of material applied to a part or product as part of an additive manufacturing process.   The valid data value MUST be an integer."@en .

:hasMaterialLayerValue a owl:DatatypeProperty ;
	rdfs:subPropertyOf :hasEventValue ;
        rdfs:range xsd:string ;
	rdfs:comment "Observed result for: Identifies the layers of material applied to a part or product as part of an additive manufacturing process.   The valid data value MUST be an integer."@en .

:ActualMaterialLayer a owl:Class ;
	rdfs:subClassOf :MaterialLayer ;
	rdfs:comment "The measured value of the data item type given by a sensor or encoder."@en .

:hasActualMaterialLayerValue a owl:DatatypeProperty ;
	rdfs:subPropertyOf :hasMaterialLayerValue ;
        rdfs:range xsd:string ;
	rdfs:comment "Observed result for: The measured value of the data item type given by a sensor or encoder."@en .

:TargetMaterialLayer a owl:Class ;
	rdfs:subClassOf :MaterialLayer ;
	rdfs:comment "The desired measure or count for a data item value."@en .

:hasTargetMaterialLayerValue a owl:DatatypeProperty ;
	rdfs:subPropertyOf :hasMaterialLayerValue ;
        rdfs:range xsd:string ;
	rdfs:comment "Observed result for: The desired measure or count for a data item value."@en .

[ rdf:type owl:AllDisjointClasses ;
        owl:members (
           :ActualMaterialLayer
           :TargetMaterialLayer
            )
        ] .

:MaterialLoad a owl:Class ;
	rdfs:subClassOf :Event ;
	rdfs:comment "Service to load a piece of material or product."@en .

:hasMaterialLoadValue a owl:DatatypeProperty ;
	rdfs:subPropertyOf :hasEventValue ;
        rdfs:range xsd:string ;
	rdfs:comment "Observed result for: Service to load a piece of material or product."@en .

:MaterialRetract a owl:Class ;
	rdfs:subClassOf :Event ;
	rdfs:comment "Service to remove or retract material or product."@en .

:hasMaterialRetractValue a owl:DatatypeProperty ;
	rdfs:subPropertyOf :hasEventValue ;
        rdfs:range xsd:string ;
	rdfs:comment "Observed result for: Service to remove or retract material or product."@en .

:MaterialUnload a owl:Class ;
	rdfs:subClassOf :Event ;
	rdfs:comment "Service to unload a piece of material or product."@en .

:hasMaterialUnloadValue a owl:DatatypeProperty ;
	rdfs:subPropertyOf :hasEventValue ;
        rdfs:range xsd:string ;
	rdfs:comment "Observed result for: Service to unload a piece of material or product."@en .

:Message a owl:Class ;
	rdfs:subClassOf :Event ;
	rdfs:comment "Any text string of information to be transferred from a piece of equipment to a client software application."@en .

:hasMessageValue a owl:DatatypeProperty ;
	rdfs:subPropertyOf :hasEventValue ;
        rdfs:range xsd:string ;
	rdfs:comment "Observed result for: Any text string of information to be transferred from a piece of equipment to a client software application."@en .

:OpenChuck a owl:Class ;
	rdfs:subClassOf :Event ;
	rdfs:comment "Service to open a chuck. "@en .

:hasOpenChuckValue a owl:DatatypeProperty ;
	rdfs:subPropertyOf :hasEventValue ;
        rdfs:range xsd:string ;
	rdfs:comment "Observed result for: Service to open a chuck. "@en .

:OpenDoor a owl:Class ;
	rdfs:subClassOf :Event ;
	rdfs:comment "Service to open a door. "@en .

:hasOpenDoorValue a owl:DatatypeProperty ;
	rdfs:subPropertyOf :hasEventValue ;
        rdfs:range xsd:string ;
	rdfs:comment "Observed result for: Service to open a door. "@en .

:OperatorId a owl:Class ;
	rdfs:subClassOf :Event ;
	rdfs:comment "The identifier of the person currently responsible for operating the piece of equipment."@en .

:hasOperatorIdValue a owl:DatatypeProperty ;
	rdfs:subPropertyOf :hasEventValue ;
        rdfs:range xsd:string ;
	rdfs:comment "Observed result for: The identifier of the person currently responsible for operating the piece of equipment."@en .

:PalletId a owl:Class ;
	rdfs:subClassOf :Event ;
	rdfs:comment "The identifier for a pallet."@en .

:hasPalletIdValue a owl:DatatypeProperty ;
	rdfs:subPropertyOf :hasEventValue ;
        rdfs:range xsd:string ;
	rdfs:comment "Observed result for: The identifier for a pallet."@en .

:PartChange a owl:Class ;
	rdfs:subClassOf :Event ;
	rdfs:comment "Service to change the part or product associated with a piece of equipment to a different part or product.  "@en .

:hasPartChangeValue a owl:DatatypeProperty ;
	rdfs:subPropertyOf :hasEventValue ;
        rdfs:range xsd:string ;
	rdfs:comment "Observed result for: Service to change the part or product associated with a piece of equipment to a different part or product.  "@en .

:PartCount a owl:Class ;
	rdfs:subClassOf :Event ;
	rdfs:comment "The count of parts produced."@en .

:hasPartCountValue a owl:DatatypeProperty ;
	rdfs:subPropertyOf :hasEventValue ;
        rdfs:range xsd:string ;
	rdfs:comment "Observed result for: The count of parts produced."@en .

:AllPartCount a owl:Class ;
	rdfs:subClassOf :PartCount ;
	rdfs:comment "The count of all the parts produced.  If the subtype is not given, this is the default."@en .

:hasAllPartCountValue a owl:DatatypeProperty ;
	rdfs:subPropertyOf :hasPartCountValue ;
        rdfs:range xsd:string ;
	rdfs:comment "Observed result for: The count of all the parts produced.  If the subtype is not given, this is the default."@en .

:GoodPartCount a owl:Class ;
	rdfs:subClassOf :PartCount ;
	rdfs:comment "Indicates the count of correct parts made."@en .

:hasGoodPartCountValue a owl:DatatypeProperty ;
	rdfs:subPropertyOf :hasPartCountValue ;
        rdfs:range xsd:string ;
	rdfs:comment "Observed result for: Indicates the count of correct parts made."@en .

:BadPartCount a owl:Class ;
	rdfs:subClassOf :PartCount ;
	rdfs:comment "Indicates the count of incorrect parts produced."@en .

:hasBadPartCountValue a owl:DatatypeProperty ;
	rdfs:subPropertyOf :hasPartCountValue ;
        rdfs:range xsd:string ;
	rdfs:comment "Observed result for: Indicates the count of incorrect parts produced."@en .

:TargetPartCount a owl:Class ;
	rdfs:subClassOf :PartCount ;
	rdfs:comment "The desired measure or count for a data item value."@en .

:hasTargetPartCountValue a owl:DatatypeProperty ;
	rdfs:subPropertyOf :hasPartCountValue ;
        rdfs:range xsd:string ;
	rdfs:comment "Observed result for: The desired measure or count for a data item value."@en .

:RemainingPartCount a owl:Class ;
	rdfs:subClassOf :PartCount ;
	rdfs:comment "Remaining measure of an object or an action."@en .

:hasRemainingPartCountValue a owl:DatatypeProperty ;
	rdfs:subPropertyOf :hasPartCountValue ;
        rdfs:range xsd:string ;
	rdfs:comment "Observed result for: Remaining measure of an object or an action."@en .

[ rdf:type owl:AllDisjointClasses ;
        owl:members (
           :AllPartCount
           :GoodPartCount
           :BadPartCount
           :TargetPartCount
           :RemainingPartCount
            )
        ] .

:PartDetect a owl:Class ;
	rdfs:subClassOf :Event ;
	rdfs:comment "An indication designating whether a part or work piece has been detected or is present.   The valid data value MUST be present or notpresent."@en .

:hasPartDetectValue a owl:DatatypeProperty ;
	rdfs:subPropertyOf :hasEventValue ;
        rdfs:range xsd:string ;
	rdfs:comment "Observed result for: An indication designating whether a part or work piece has been detected or is present.   The valid data value MUST be present or notpresent."@en .

:PartId a owl:Class ;
	rdfs:subClassOf :Event ;
	rdfs:comment "An identifier of a part in a manufacturing operation."@en .

:hasPartIdValue a owl:DatatypeProperty ;
	rdfs:subPropertyOf :hasEventValue ;
        rdfs:range xsd:string ;
	rdfs:comment "Observed result for: An identifier of a part in a manufacturing operation."@en .

:PartNumber a owl:Class ;
	rdfs:subClassOf :Event ;
	rdfs:comment "An identifier of a part or product moving through the manufacturing process.  The valid data value must be a text string. "@en .

:hasPartNumberValue a owl:DatatypeProperty ;
	rdfs:subPropertyOf :hasEventValue ;
        rdfs:range xsd:string ;
	rdfs:comment "Observed result for: An identifier of a part or product moving through the manufacturing process.  The valid data value must be a text string. "@en .

:PathFeedrateOverride a owl:Class ;
	rdfs:subClassOf :Event ;
	rdfs:comment "The value of a signal or calculation issued to adjust the feedrate for the axes associated with a path component that may represent a single axis or the coordinated movement of multiple axes."@en .

:hasPathFeedrateOverrideValue a owl:DatatypeProperty ;
	rdfs:subPropertyOf :hasEventValue ;
        rdfs:range xsd:string ;
	rdfs:comment "Observed result for: The value of a signal or calculation issued to adjust the feedrate for the axes associated with a path component that may represent a single axis or the coordinated movement of multiple axes."@en .

:JogPathFeedrateOverride a owl:Class ;
	rdfs:subClassOf :PathFeedrateOverride ;
	rdfs:comment "The feedrate specified by a logic or motion program, by a pre-set value, or set by a switch as the feedrate for the axes. "@en .

:hasJogPathFeedrateOverrideValue a owl:DatatypeProperty ;
	rdfs:subPropertyOf :hasPathFeedrateOverrideValue ;
        rdfs:range xsd:string ;
	rdfs:comment "Observed result for: The feedrate specified by a logic or motion program, by a pre-set value, or set by a switch as the feedrate for the axes. "@en .

:ProgrammedPathFeedrateOverride a owl:Class ;
	rdfs:subClassOf :PathFeedrateOverride ;
	rdfs:comment "The value of a signal or calculation specified by a logic or motion program or set by a switch."@en .

:hasProgrammedPathFeedrateOverrideValue a owl:DatatypeProperty ;
	rdfs:subPropertyOf :hasPathFeedrateOverrideValue ;
        rdfs:range xsd:string ;
	rdfs:comment "Observed result for: The value of a signal or calculation specified by a logic or motion program or set by a switch."@en .

:RapidPathFeedrateOverride a owl:Class ;
	rdfs:subClassOf :PathFeedrateOverride ;
	rdfs:comment "The value of a signal or calculation issued to adjust the feedrate of a component or composition that is operating in a rapid positioning mode."@en .

:hasRapidPathFeedrateOverrideValue a owl:DatatypeProperty ;
	rdfs:subPropertyOf :hasPathFeedrateOverrideValue ;
        rdfs:range xsd:string ;
	rdfs:comment "Observed result for: The value of a signal or calculation issued to adjust the feedrate of a component or composition that is operating in a rapid positioning mode."@en .

[ rdf:type owl:AllDisjointClasses ;
        owl:members (
           :JogPathFeedrateOverride
           :ProgrammedPathFeedrateOverride
           :RapidPathFeedrateOverride
            )
        ] .

:PathMode a owl:Class ;
    owl:equivalentClass [ owl:intersectionOf ( :State 
            [ rdf:type owl:Class ;
                owl:oneOf (
                    :INDEPENDENT
                    :MASTER
                    :SYNCHRONOUS
                    :MIRROR
                    )
                ]
            ) ;
            a owl:Class
        ] .

:hasPathMode a owl:ObjectProperty ;
	rdfs:subPropertyOf :hasState ;
        rdfs:range :PathMode ;
	rdfs:comment "Observed result for: Describes the operational relationship between a path structural element and another path structural element for pieces of equipment comprised of multiple logical groupings of controlled axes or other logical operations."@en .

:PowerState a owl:Class ;
    owl:equivalentClass [ owl:intersectionOf ( :State 
            [ rdf:type owl:Class ;
                owl:oneOf (
                    :ON
                    :OFF
                    )
                ]
            ) ;
            a owl:Class
        ] .

:hasPowerState a owl:ObjectProperty ;
	rdfs:subPropertyOf :hasState ;
        rdfs:range :PowerState ;
	rdfs:comment "Observed result for: The indication of the status of the source of energy for a structural element to allow it to perform its intended function or the state of an enabling signal providing permission for the structural element to perform its functions."@en .

:LinePowerState a owl:Class ;
	rdfs:subClassOf :PowerState ;
	rdfs:comment "The state of the power source for the structural element."@en .

:hasLinePowerState a owl:ObjectProperty ;
	rdfs:subPropertyOf :hasPowerState ;
        rdfs:range :PowerState ;
	rdfs:comment "Observed result for: The state of the power source for the structural element."@en .

:ControlPowerState a owl:Class ;
	rdfs:subClassOf :PowerState ;
	rdfs:comment "The state of the enabling signal or control logic that enables or disables the function or operation of the structural element."@en .

:hasControlPowerState a owl:ObjectProperty ;
	rdfs:subPropertyOf :hasPowerState ;
        rdfs:range :PowerState ;
	rdfs:comment "Observed result for: The state of the enabling signal or control logic that enables or disables the function or operation of the structural element."@en .

[ rdf:type owl:AllDisjointClasses ;
        owl:members (
           :LinePowerState
           :ControlPowerState
            )
        ] .

:PowerStatus a owl:Class ;
	rdfs:subClassOf :Event ;
	rdfs:comment "DEPRECATED in Version 1.1.0."@en .

:hasPowerStatusValue a owl:DatatypeProperty ;
	rdfs:subPropertyOf :hasEventValue ;
        rdfs:range xsd:string ;
	rdfs:comment "Observed result for: DEPRECATED in Version 1.1.0."@en .

:ProcessTime a owl:Class ;
	rdfs:subClassOf :Event ;
	rdfs:comment "The time and date associated with an activity or event.   processtime event MUST be reported in ISO 8601 format."@en .

:hasProcessTimeValue a owl:DatatypeProperty ;
	rdfs:subPropertyOf :hasEventValue ;
        rdfs:range xsd:string ;
	rdfs:comment "Observed result for: The time and date associated with an activity or event.   processtime event MUST be reported in ISO 8601 format."@en .

:StartProcessTime a owl:Class ;
	rdfs:subClassOf :ProcessTime ;
	rdfs:comment "The time and date associated with the beginning of an activity or event."@en .

:hasStartProcessTimeValue a owl:DatatypeProperty ;
	rdfs:subPropertyOf :hasProcessTimeValue ;
        rdfs:range xsd:string ;
	rdfs:comment "Observed result for: The time and date associated with the beginning of an activity or event."@en .

:CompleteProcessTime a owl:Class ;
	rdfs:subClassOf :ProcessTime ;
	rdfs:comment "Completion of an action."@en .

:hasCompleteProcessTimeValue a owl:DatatypeProperty ;
	rdfs:subPropertyOf :hasProcessTimeValue ;
        rdfs:range xsd:string ;
	rdfs:comment "Observed result for: Completion of an action."@en .

:TargetCompletionProcessTime a owl:Class ;
	rdfs:subClassOf :ProcessTime ;
	rdfs:comment "The projected time and date associated with the end or completion of an activity or event."@en .

:hasTargetCompletionProcessTimeValue a owl:DatatypeProperty ;
	rdfs:subPropertyOf :hasProcessTimeValue ;
        rdfs:range xsd:string ;
	rdfs:comment "Observed result for: The projected time and date associated with the end or completion of an activity or event."@en .

[ rdf:type owl:AllDisjointClasses ;
        owl:members (
           :StartProcessTime
           :CompleteProcessTime
           :TargetCompletionProcessTime
            )
        ] .

:Program a owl:Class ;
	rdfs:subClassOf :Event ;
	rdfs:comment "The name of the logic or motion program being executed by the controller component."@en .

:hasProgramValue a owl:DatatypeProperty ;
	rdfs:subPropertyOf :hasEventValue ;
        rdfs:range xsd:string ;
	rdfs:comment "Observed result for: The name of the logic or motion program being executed by the controller component."@en .

:ProgramComment a owl:Class ;
	rdfs:subClassOf :Event ;
	rdfs:comment "A comment or non-executable statement in the control program. The valid data value must be a text string."@en .

:hasProgramCommentValue a owl:DatatypeProperty ;
	rdfs:subPropertyOf :hasEventValue ;
        rdfs:range xsd:string ;
	rdfs:comment "Observed result for: A comment or non-executable statement in the control program. The valid data value must be a text string."@en .

:ProgramEdit a owl:Class ;
    owl:equivalentClass [ owl:intersectionOf ( :State 
            [ rdf:type owl:Class ;
                owl:oneOf (
                    :ACTIVE
                    :READY
                    :NOT_READY
                    )
                ]
            ) ;
            a owl:Class
        ] .

:hasProgramEdit a owl:ObjectProperty ;
	rdfs:subPropertyOf :hasState ;
        rdfs:range :ProgramEdit ;
	rdfs:comment "Observed result for: An indication of the status of the controller components program editing mode.  On many controls, a program can be edited while another program is currently being executed."@en .

:ProgramEditName a owl:Class ;
	rdfs:subClassOf :Event ;
	rdfs:comment "The name of the program being edited.  This is used in conjunction with programedit event when in active value state.  The valid data value must be a text string."@en .

:hasProgramEditNameValue a owl:DatatypeProperty ;
	rdfs:subPropertyOf :hasEventValue ;
        rdfs:range xsd:string ;
	rdfs:comment "Observed result for: The name of the program being edited.  This is used in conjunction with programedit event when in active value state.  The valid data value must be a text string."@en .

:ProgramHeader a owl:Class ;
	rdfs:subClassOf :Event ;
	rdfs:comment "The non-executable header section of the control program."@en .

:hasProgramHeaderValue a owl:DatatypeProperty ;
	rdfs:subPropertyOf :hasEventValue ;
        rdfs:range xsd:string ;
	rdfs:comment "Observed result for: The non-executable header section of the control program."@en .

:ProgramLocation a owl:Class ;
	rdfs:subClassOf :Event ;
	rdfs:comment "The Uniform Resource Identifier (URI) for the source file associated with program event."@en .

:hasProgramLocationValue a owl:DatatypeProperty ;
	rdfs:subPropertyOf :hasEventValue ;
        rdfs:range xsd:string ;
	rdfs:comment "Observed result for: The Uniform Resource Identifier (URI) for the source file associated with program event."@en .

:ScheduleProgramLocation a owl:Class ;
	rdfs:subClassOf :ProgramLocation ;
	rdfs:comment "The identity of a control program that is used to specify the order of execution of other programs."@en .

:hasScheduleProgramLocationValue a owl:DatatypeProperty ;
	rdfs:subPropertyOf :hasProgramLocationValue ;
        rdfs:range xsd:string ;
	rdfs:comment "Observed result for: The identity of a control program that is used to specify the order of execution of other programs."@en .

:MainProgramLocation a owl:Class ;
	rdfs:subClassOf :ProgramLocation ;
	rdfs:comment "The identity of the primary logic or motion program currently being executed. It is the starting nest level in a call structure and may contain calls to sub programs."@en .

:hasMainProgramLocationValue a owl:DatatypeProperty ;
	rdfs:subPropertyOf :hasProgramLocationValue ;
        rdfs:range xsd:string ;
	rdfs:comment "Observed result for: The identity of the primary logic or motion program currently being executed. It is the starting nest level in a call structure and may contain calls to sub programs."@en .

:ActiveProgramLocation a owl:Class ;
	rdfs:subClassOf :ProgramLocation ;
	rdfs:comment "The value of the data entity that is engaging."@en .

:hasActiveProgramLocationValue a owl:DatatypeProperty ;
	rdfs:subPropertyOf :hasProgramLocationValue ;
        rdfs:range xsd:string ;
	rdfs:comment "Observed result for: The value of the data entity that is engaging."@en .

[ rdf:type owl:AllDisjointClasses ;
        owl:members (
           :ScheduleProgramLocation
           :MainProgramLocation
           :ActiveProgramLocation
            )
        ] .

:ProgramLocationType a owl:Class ;
	rdfs:subClassOf :Event ;
	rdfs:comment "Defines whether the logic or motion program defined by program event is being executed from the local memory of the controller or from an outside source.   The valid data value MUST be local or external."@en .

:hasProgramLocationTypeValue a owl:DatatypeProperty ;
	rdfs:subPropertyOf :hasEventValue ;
        rdfs:range xsd:string ;
	rdfs:comment "Observed result for: Defines whether the logic or motion program defined by program event is being executed from the local memory of the controller or from an outside source.   The valid data value MUST be local or external."@en .

:ScheduleProgramLocationType a owl:Class ;
	rdfs:subClassOf :ProgramLocationType ;
	rdfs:comment "The identity of a control program that is used to specify the order of execution of other programs."@en .

:hasScheduleProgramLocationTypeValue a owl:DatatypeProperty ;
	rdfs:subPropertyOf :hasProgramLocationTypeValue ;
        rdfs:range xsd:string ;
	rdfs:comment "Observed result for: The identity of a control program that is used to specify the order of execution of other programs."@en .

:MainProgramLocationType a owl:Class ;
	rdfs:subClassOf :ProgramLocationType ;
	rdfs:comment "The identity of the primary logic or motion program currently being executed. It is the starting nest level in a call structure and may contain calls to sub programs."@en .

:hasMainProgramLocationTypeValue a owl:DatatypeProperty ;
	rdfs:subPropertyOf :hasProgramLocationTypeValue ;
        rdfs:range xsd:string ;
	rdfs:comment "Observed result for: The identity of the primary logic or motion program currently being executed. It is the starting nest level in a call structure and may contain calls to sub programs."@en .

:ActiveProgramLocationType a owl:Class ;
	rdfs:subClassOf :ProgramLocationType ;
	rdfs:comment "The value of the data entity that is engaging."@en .

:hasActiveProgramLocationTypeValue a owl:DatatypeProperty ;
	rdfs:subPropertyOf :hasProgramLocationTypeValue ;
        rdfs:range xsd:string ;
	rdfs:comment "Observed result for: The value of the data entity that is engaging."@en .

[ rdf:type owl:AllDisjointClasses ;
        owl:members (
           :ScheduleProgramLocationType
           :MainProgramLocationType
           :ActiveProgramLocationType
            )
        ] .

:ProgramNestLevel a owl:Class ;
	rdfs:subClassOf :Event ;
	rdfs:comment "An indication of the nesting level within a control program that is associated with the code or instructions that is currently being executed.   If an Initial Value is not defined, the nesting level associated with the highest or initial nesting level of the program MUST default to zero (0).   The value reported for programnestlevel event MUST be an integer."@en .

:hasProgramNestLevelValue a owl:DatatypeProperty ;
	rdfs:subPropertyOf :hasEventValue ;
        rdfs:range xsd:string ;
	rdfs:comment "Observed result for: An indication of the nesting level within a control program that is associated with the code or instructions that is currently being executed.   If an Initial Value is not defined, the nesting level associated with the highest or initial nesting level of the program MUST default to zero (0).   The value reported for programnestlevel event MUST be an integer."@en .

:RotaryMode a owl:Class ;
    owl:equivalentClass [ owl:intersectionOf ( :State 
            [ rdf:type owl:Class ;
                owl:oneOf (
                    :SPINDLE
                    :INDEX
                    :CONTOUR
                    )
                ]
            ) ;
            a owl:Class
        ] .

:hasRotaryMode a owl:ObjectProperty ;
	rdfs:subPropertyOf :hasState ;
        rdfs:range :RotaryMode ;
	rdfs:comment "Observed result for: The current operating mode for a rotary type axis."@en .

:RotaryVelocityOverride a owl:Class ;
	rdfs:subClassOf :Event ;
	rdfs:comment "The value of a command issued to adjust the programmed velocity for a rotary type axis. This command represents a percentage change to the velocity calculated by a logic or motion program or set by a switch for a rotary type axis."@en .

:hasRotaryVelocityOverrideValue a owl:DatatypeProperty ;
	rdfs:subPropertyOf :hasEventValue ;
        rdfs:range xsd:string ;
	rdfs:comment "Observed result for: The value of a command issued to adjust the programmed velocity for a rotary type axis. This command represents a percentage change to the velocity calculated by a logic or motion program or set by a switch for a rotary type axis."@en .

:SerialNumber a owl:Class ;
	rdfs:subClassOf :Event ;
	rdfs:comment "The serial number associated with a component, asset mtconnectassets, or device. The valid data value must be a text string."@en .

:hasSerialNumberValue a owl:DatatypeProperty ;
	rdfs:subPropertyOf :hasEventValue ;
        rdfs:range xsd:string ;
	rdfs:comment "Observed result for: The serial number associated with a component, asset mtconnectassets, or device. The valid data value must be a text string."@en .

:SpindleInterlock a owl:Class ;
    owl:equivalentClass [ owl:intersectionOf ( :State 
            [ rdf:type owl:Class ;
                owl:oneOf (
                    :ACTIVE
                    :INACTIVE
                    )
                ]
            ) ;
            a owl:Class
        ] .

:hasSpindleInterlock a owl:ObjectProperty ;
	rdfs:subPropertyOf :hasState ;
        rdfs:range :SpindleInterlock ;
	rdfs:comment "Observed result for: An indication of the status of the spindle for a piece of equipment when power has been removed and it is free to rotate."@en .

:ToolAssetId a owl:Class ;
	rdfs:subClassOf :Event ;
	rdfs:comment "The identifier of an individual tool asset.The valid data value must be a text string."@en .

:hasToolAssetIdValue a owl:DatatypeProperty ;
	rdfs:subPropertyOf :hasEventValue ;
        rdfs:range xsd:string ;
	rdfs:comment "Observed result for: The identifier of an individual tool asset.The valid data value must be a text string."@en .

:ToolGroup a owl:Class ;
	rdfs:subClassOf :Event ;
	rdfs:comment "An identifier for the tool group associated with a specific tool. Commonly used to designate spare tools."@en .

:hasToolGroupValue a owl:DatatypeProperty ;
	rdfs:subPropertyOf :hasEventValue ;
        rdfs:range xsd:string ;
	rdfs:comment "Observed result for: An identifier for the tool group associated with a specific tool. Commonly used to designate spare tools."@en .

:ToolId a owl:Class ;
	rdfs:subClassOf :Event ;
	rdfs:comment "DEPRECATED in Version 1.2.0.   See toolassetid event. The identifier of the tool currently in use for a given path."@en .

:hasToolIdValue a owl:DatatypeProperty ;
	rdfs:subPropertyOf :hasEventValue ;
        rdfs:range xsd:string ;
	rdfs:comment "Observed result for: DEPRECATED in Version 1.2.0.   See toolassetid event. The identifier of the tool currently in use for a given path."@en .

:ToolNumber a owl:Class ;
	rdfs:subClassOf :Event ;
	rdfs:comment "The identifier assigned by the controller component to a cutting tool when in use by a piece of equipment.  The valid data value must be a text string."@en .

:hasToolNumberValue a owl:DatatypeProperty ;
	rdfs:subPropertyOf :hasEventValue ;
        rdfs:range xsd:string ;
	rdfs:comment "Observed result for: The identifier assigned by the controller component to a cutting tool when in use by a piece of equipment.  The valid data value must be a text string."@en .

:ToolOffset a owl:Class ;
	rdfs:subClassOf :Event ;
	rdfs:comment "A reference to the tool offset variables applied to the active cutting tool associated with a path in a controller type component."@en .

:hasToolOffsetValue a owl:DatatypeProperty ;
	rdfs:subPropertyOf :hasEventValue ;
        rdfs:range xsd:string ;
	rdfs:comment "Observed result for: A reference to the tool offset variables applied to the active cutting tool associated with a path in a controller type component."@en .

:RadialToolOffset a owl:Class ;
	rdfs:subClassOf :ToolOffset ;
	rdfs:comment "A reference to a radial type tool offset variable."@en .

:hasRadialToolOffsetValue a owl:DatatypeProperty ;
	rdfs:subPropertyOf :hasToolOffsetValue ;
        rdfs:range xsd:string ;
	rdfs:comment "Observed result for: A reference to a radial type tool offset variable."@en .

:LengthToolOffset a owl:Class ;
	rdfs:subClassOf :ToolOffset ;
	rdfs:comment "A reference to a length type tool offset variable."@en .

:hasLengthToolOffsetValue a owl:DatatypeProperty ;
	rdfs:subPropertyOf :hasToolOffsetValue ;
        rdfs:range xsd:string ;
	rdfs:comment "Observed result for: A reference to a length type tool offset variable."@en .

[ rdf:type owl:AllDisjointClasses ;
        owl:members (
           :RadialToolOffset
           :LengthToolOffset
            )
        ] .

:User a owl:Class ;
	rdfs:subClassOf :Event ;
	rdfs:comment "The identifier of the person currently responsible for operating the piece of equipment."@en .

:hasUserValue a owl:DatatypeProperty ;
	rdfs:subPropertyOf :hasEventValue ;
        rdfs:range xsd:string ;
	rdfs:comment "Observed result for: The identifier of the person currently responsible for operating the piece of equipment."@en .

:OperatorUser a owl:Class ;
	rdfs:subClassOf :User ;
	rdfs:comment "The identifier of the person currently responsible for operating the piece of equipment."@en .

:hasOperatorUserValue a owl:DatatypeProperty ;
	rdfs:subPropertyOf :hasUserValue ;
        rdfs:range xsd:string ;
	rdfs:comment "Observed result for: The identifier of the person currently responsible for operating the piece of equipment."@en .

:MaintenanceUser a owl:Class ;
	rdfs:subClassOf :User ;
	rdfs:comment "Action related to maintenance on the piece of equipment."@en .

:hasMaintenanceUserValue a owl:DatatypeProperty ;
	rdfs:subPropertyOf :hasUserValue ;
        rdfs:range xsd:string ;
	rdfs:comment "Observed result for: Action related to maintenance on the piece of equipment."@en .

:SetUpUser a owl:Class ;
	rdfs:subClassOf :User ;
	rdfs:comment "The identifier of the person currently responsible for preparing a piece of equipment for production or restoring the piece of equipment to a neutral state after production."@en .

:hasSetUpUserValue a owl:DatatypeProperty ;
	rdfs:subPropertyOf :hasUserValue ;
        rdfs:range xsd:string ;
	rdfs:comment "Observed result for: The identifier of the person currently responsible for preparing a piece of equipment for production or restoring the piece of equipment to a neutral state after production."@en .

[ rdf:type owl:AllDisjointClasses ;
        owl:members (
           :OperatorUser
           :MaintenanceUser
           :SetUpUser
            )
        ] .

:Variable a owl:Class ;
	rdfs:subClassOf :Event ;
	rdfs:comment " A data value whose meaning may change over time due to changes in the opertion of a piece of equipment or the process being executed on that piece of equipment."@en .

:hasVariableValue a owl:DatatypeProperty ;
	rdfs:subPropertyOf :hasEventValue ;
        rdfs:range xsd:string ;
	rdfs:comment "Observed result for:  A data value whose meaning may change over time due to changes in the opertion of a piece of equipment or the process being executed on that piece of equipment."@en .

:WaitState a owl:Class ;
	rdfs:subClassOf :Event ;
	rdfs:comment "An indication of the reason that execution event is reporting a value of wait.   The valid data value MUST be poweringup, poweringdown, partload, partunload, toolload, toolunload, materialload event, materialunload event, secondaryprocess, pausing, or resuming."@en .

:hasWaitStateValue a owl:DatatypeProperty ;
	rdfs:subPropertyOf :hasEventValue ;
        rdfs:range xsd:string ;
	rdfs:comment "Observed result for: An indication of the reason that execution event is reporting a value of wait.   The valid data value MUST be poweringup, poweringdown, partload, partunload, toolload, toolunload, materialload event, materialunload event, secondaryprocess, pausing, or resuming."@en .

:WireId a owl:Class ;
	rdfs:subClassOf :Event ;
	rdfs:comment "A string like piece or filament of relatively rigid or flexible material provided in a variety of diameters."@en .

:hasWireIdValue a owl:DatatypeProperty ;
	rdfs:subPropertyOf :hasEventValue ;
        rdfs:range xsd:string ;
	rdfs:comment "Observed result for: A string like piece or filament of relatively rigid or flexible material provided in a variety of diameters."@en .

:WorkholdingId a owl:Class ;
	rdfs:subClassOf :Event ;
	rdfs:comment "The identifier for the current workholding or part clamp in use by a piece of equipment.  The valid data value must be a text string."@en .

:hasWorkholdingIdValue a owl:DatatypeProperty ;
	rdfs:subPropertyOf :hasEventValue ;
        rdfs:range xsd:string ;
	rdfs:comment "Observed result for: The identifier for the current workholding or part clamp in use by a piece of equipment.  The valid data value must be a text string."@en .

:WorkOffset a owl:Class ;
	rdfs:subClassOf :Event ;
	rdfs:comment "A reference to the offset variables for a work piece or part associated with a path in a controller type component."@en .

:hasWorkOffsetValue a owl:DatatypeProperty ;
	rdfs:subPropertyOf :hasEventValue ;
        rdfs:range xsd:string ;
	rdfs:comment "Observed result for: A reference to the offset variables for a work piece or part associated with a path in a controller type component."@en .

[ rdf:type owl:AllDisjointClasses ;
        owl:members (
           :ActiveAxes
           :Alarm
           :AssetChanged
           :AssetRemoved
           :AxisFeedrateOverride
           :Block
           :BlockCount
           :CloseChuck
           :CloseDoor
           :Code
           :CompositionState
           :CoupledAxes
           :DateCode
           :DeviceUuid
           :Direction
           :Hardness
           :Line
           :LineLabel
           :LineNumber
           :Material
           :MaterialChange
           :MaterialFeed
           :MaterialLayer
           :MaterialLoad
           :MaterialRetract
           :MaterialUnload
           :Message
           :OpenChuck
           :OpenDoor
           :OperatorId
           :PalletId
           :PartChange
           :PartCount
           :PartDetect
           :PartId
           :PartNumber
           :PathFeedrateOverride
           :PowerStatus
           :ProcessTime
           :Program
           :ProgramComment
           :ProgramEditName
           :ProgramHeader
           :ProgramLocation
           :ProgramLocationType
           :ProgramNestLevel
           :RotaryVelocityOverride
           :SerialNumber
           :ToolAssetId
           :ToolGroup
           :ToolId
           :ToolNumber
           :ToolOffset
           :User
           :Variable
           :WaitState
           :WireId
           :WorkholdingId
           :WorkOffset
            )
        ] .

:Acceleration a owl:Class ;
	rdfs:subClassOf :Sample ;
	rdfs:comment "The measurement of the rate of change of velocity.. The units are MILLIMETER/SECOND^2."@en .

:hasAccelerationValue a owl:DatatypeProperty ;
	rdfs:subPropertyOf :hasSampledValue ;
        rdfs:range xsd:float ;
	rdfs:comment "Observed result for: The measurement of the rate of change of velocity.. The units are MILLIMETER/SECOND^2."@en .

:AccumulatedTime a owl:Class ;
	rdfs:subClassOf :Sample ;
	rdfs:comment "The measurement of accumulated time for an activity or event.. The units are SECOND."@en .

:hasAccumulatedTimeValue a owl:DatatypeProperty ;
	rdfs:subPropertyOf :hasSampledValue ;
        rdfs:range xsd:float ;
	rdfs:comment "Observed result for: The measurement of accumulated time for an activity or event.. The units are SECOND."@en .

:Amperage a owl:Class ;
	rdfs:subClassOf :Sample ;
	rdfs:comment "The measurement of electrical current.. The units are AMPERE."@en .

:hasAmperageValue a owl:DatatypeProperty ;
	rdfs:subPropertyOf :hasSampledValue ;
        rdfs:range xsd:float ;
	rdfs:comment "Observed result for: The measurement of electrical current.. The units are AMPERE."@en .

:AlternatingAmperage a owl:Class ;
	rdfs:subClassOf :Amperage ;
	rdfs:comment "The measurement of alternating voltage or current.   If not specified further in statistic, defaults to RMS voltage. "@en .

:hasAlternatingAmperageValue a owl:DatatypeProperty ;
	rdfs:subPropertyOf :hasAmperageValue ;
        rdfs:range xsd:float ;
	rdfs:comment "Observed result for: The measurement of alternating voltage or current.   If not specified further in statistic, defaults to RMS voltage. "@en .

:DirectAmperage a owl:Class ;
	rdfs:subClassOf :Amperage ;
	rdfs:comment "The measurement of DC current or voltage."@en .

:hasDirectAmperageValue a owl:DatatypeProperty ;
	rdfs:subPropertyOf :hasAmperageValue ;
        rdfs:range xsd:float ;
	rdfs:comment "Observed result for: The measurement of DC current or voltage."@en .

:ActualAmperage a owl:Class ;
	rdfs:subClassOf :Amperage ;
	rdfs:comment "The measured value of the data item type given by a sensor or encoder."@en .

:hasActualAmperageValue a owl:DatatypeProperty ;
	rdfs:subPropertyOf :hasAmperageValue ;
        rdfs:range xsd:float ;
	rdfs:comment "Observed result for: The measured value of the data item type given by a sensor or encoder."@en .

:TargetAmperage a owl:Class ;
	rdfs:subClassOf :Amperage ;
	rdfs:comment "The desired measure or count for a data item value."@en .

:hasTargetAmperageValue a owl:DatatypeProperty ;
	rdfs:subPropertyOf :hasAmperageValue ;
        rdfs:range xsd:float ;
	rdfs:comment "Observed result for: The desired measure or count for a data item value."@en .

[ rdf:type owl:AllDisjointClasses ;
        owl:members (
           :AlternatingAmperage
           :DirectAmperage
           :ActualAmperage
           :TargetAmperage
            )
        ] .

:Angle a owl:Class ;
	rdfs:subClassOf :Sample ;
	rdfs:comment "The measurement of angular position.. The units are DEGREE."@en .

:hasAngleValue a owl:DatatypeProperty ;
	rdfs:subPropertyOf :hasSampledValue ;
        rdfs:range xsd:float ;
	rdfs:comment "Observed result for: The measurement of angular position.. The units are DEGREE."@en .

:CommandedAngle a owl:Class ;
	rdfs:subClassOf :Angle ;
	rdfs:comment "A value specified by the controller type component."@en .

:hasCommandedAngleValue a owl:DatatypeProperty ;
	rdfs:subPropertyOf :hasAngleValue ;
        rdfs:range xsd:float ;
	rdfs:comment "Observed result for: A value specified by the controller type component."@en .

:ActualAngle a owl:Class ;
	rdfs:subClassOf :Angle ;
	rdfs:comment "The measured value of the data item type given by a sensor or encoder."@en .

:hasActualAngleValue a owl:DatatypeProperty ;
	rdfs:subPropertyOf :hasAngleValue ;
        rdfs:range xsd:float ;
	rdfs:comment "Observed result for: The measured value of the data item type given by a sensor or encoder."@en .

[ rdf:type owl:AllDisjointClasses ;
        owl:members (
           :CommandedAngle
           :ActualAngle
            )
        ] .

:AngularAcceleration a owl:Class ;
	rdfs:subClassOf :Sample ;
	rdfs:comment "The measurement rate of change of angular velocity.. The units are DEGREE/SECOND^2."@en .

:hasAngularAccelerationValue a owl:DatatypeProperty ;
	rdfs:subPropertyOf :hasSampledValue ;
        rdfs:range xsd:float ;
	rdfs:comment "Observed result for: The measurement rate of change of angular velocity.. The units are DEGREE/SECOND^2."@en .

:AngularVelocity a owl:Class ;
	rdfs:subClassOf :Sample ;
	rdfs:comment "The measurement of the rate of change of angular position.. The units are DEGREE/SECOND."@en .

:hasAngularVelocityValue a owl:DatatypeProperty ;
	rdfs:subPropertyOf :hasSampledValue ;
        rdfs:range xsd:float ;
	rdfs:comment "Observed result for: The measurement of the rate of change of angular position.. The units are DEGREE/SECOND."@en .

:AxisFeedrate a owl:Class ;
	rdfs:subClassOf :Sample ;
	rdfs:comment "The measurement of the feedrate of a linear axis.. The units are MILLIMETER/SECOND."@en .

:hasAxisFeedrateValue a owl:DatatypeProperty ;
	rdfs:subPropertyOf :hasSampledValue ;
        rdfs:range xsd:float ;
	rdfs:comment "Observed result for: The measurement of the feedrate of a linear axis.. The units are MILLIMETER/SECOND."@en .

:ActualAxisFeedrate a owl:Class ;
	rdfs:subClassOf :AxisFeedrate ;
	rdfs:comment "The measured value of the data item type given by a sensor or encoder."@en .

:hasActualAxisFeedrateValue a owl:DatatypeProperty ;
	rdfs:subPropertyOf :hasAxisFeedrateValue ;
        rdfs:range xsd:float ;
	rdfs:comment "Observed result for: The measured value of the data item type given by a sensor or encoder."@en .

:CommandedAxisFeedrate a owl:Class ;
	rdfs:subClassOf :AxisFeedrate ;
	rdfs:comment "A value specified by the controller type component."@en .

:hasCommandedAxisFeedrateValue a owl:DatatypeProperty ;
	rdfs:subPropertyOf :hasAxisFeedrateValue ;
        rdfs:range xsd:float ;
	rdfs:comment "Observed result for: A value specified by the controller type component."@en .

:JogAxisFeedrate a owl:Class ;
	rdfs:subClassOf :AxisFeedrate ;
	rdfs:comment "The feedrate specified by a logic or motion program, by a pre-set value, or set by a switch as the feedrate for the axes. "@en .

:hasJogAxisFeedrateValue a owl:DatatypeProperty ;
	rdfs:subPropertyOf :hasAxisFeedrateValue ;
        rdfs:range xsd:float ;
	rdfs:comment "Observed result for: The feedrate specified by a logic or motion program, by a pre-set value, or set by a switch as the feedrate for the axes. "@en .

:ProgrammedAxisFeedrate a owl:Class ;
	rdfs:subClassOf :AxisFeedrate ;
	rdfs:comment "The value of a signal or calculation specified by a logic or motion program or set by a switch."@en .

:hasProgrammedAxisFeedrateValue a owl:DatatypeProperty ;
	rdfs:subPropertyOf :hasAxisFeedrateValue ;
        rdfs:range xsd:float ;
	rdfs:comment "Observed result for: The value of a signal or calculation specified by a logic or motion program or set by a switch."@en .

:RapidAxisFeedrate a owl:Class ;
	rdfs:subClassOf :AxisFeedrate ;
	rdfs:comment "The value of a signal or calculation issued to adjust the feedrate of a component or composition that is operating in a rapid positioning mode."@en .

:hasRapidAxisFeedrateValue a owl:DatatypeProperty ;
	rdfs:subPropertyOf :hasAxisFeedrateValue ;
        rdfs:range xsd:float ;
	rdfs:comment "Observed result for: The value of a signal or calculation issued to adjust the feedrate of a component or composition that is operating in a rapid positioning mode."@en .

:OverrideAxisFeedrate a owl:Class ;
	rdfs:subClassOf :AxisFeedrate ;
	rdfs:comment "DEPRECATED: The operators overridden value."@en .

:hasOverrideAxisFeedrateValue a owl:DatatypeProperty ;
	rdfs:subPropertyOf :hasAxisFeedrateValue ;
        rdfs:range xsd:float ;
	rdfs:comment "Observed result for: DEPRECATED: The operators overridden value."@en .

[ rdf:type owl:AllDisjointClasses ;
        owl:members (
           :ActualAxisFeedrate
           :CommandedAxisFeedrate
           :JogAxisFeedrate
           :ProgrammedAxisFeedrate
           :RapidAxisFeedrate
           :OverrideAxisFeedrate
            )
        ] .

:CapacityFluid a owl:Class ;
	rdfs:subClassOf :Sample ;
	rdfs:comment "The fluid capacity of an object or container.. The units are MILLILITER."@en .

:hasCapacityFluidValue a owl:DatatypeProperty ;
	rdfs:subPropertyOf :hasSampledValue ;
        rdfs:range xsd:float ;
	rdfs:comment "Observed result for: The fluid capacity of an object or container.. The units are MILLILITER."@en .

:CapacitySpatial a owl:Class ;
	rdfs:subClassOf :Sample ;
	rdfs:comment "The geometric capacity of an object or container.. The units are CUBIC_MILLIMETER."@en .

:hasCapacitySpatialValue a owl:DatatypeProperty ;
	rdfs:subPropertyOf :hasSampledValue ;
        rdfs:range xsd:float ;
	rdfs:comment "Observed result for: The geometric capacity of an object or container.. The units are CUBIC_MILLIMETER."@en .

:ClockTime a owl:Class ;
	rdfs:subClassOf :Sample ;
	rdfs:comment "The value provided by a timing device at a specific point in time.. The units are yyyy-mm-ddthh:mm:ss.ffff."@en .

:hasClockTimeValue a owl:DatatypeProperty ;
	rdfs:subPropertyOf :hasSampledValue ;
        rdfs:range xsd:float ;
	rdfs:comment "Observed result for: The value provided by a timing device at a specific point in time.. The units are yyyy-mm-ddthh:mm:ss.ffff."@en .

:Concentration a owl:Class ;
	rdfs:subClassOf :Sample ;
	rdfs:comment "The measurement of the percentage of one component within a mixture of components. The units are PERCENT."@en .

:hasConcentrationValue a owl:DatatypeProperty ;
	rdfs:subPropertyOf :hasSampledValue ;
        rdfs:range xsd:float ;
	rdfs:comment "Observed result for: The measurement of the percentage of one component within a mixture of components. The units are PERCENT."@en .

:Conductivity a owl:Class ;
	rdfs:subClassOf :Sample ;
	rdfs:comment "The measurement of the ability of a material to conduct electricity.. The units are SIEMENS/METER."@en .

:hasConductivityValue a owl:DatatypeProperty ;
	rdfs:subPropertyOf :hasSampledValue ;
        rdfs:range xsd:float ;
	rdfs:comment "Observed result for: The measurement of the ability of a material to conduct electricity.. The units are SIEMENS/METER."@en .

:CuttingSpeed a owl:Class ;
	rdfs:subClassOf :Sample ;
	rdfs:comment " The speed difference (relative velocity) between the cutting mechanism and the surface of the workpiece it is operating on.. The units are MILLIMETER/SECOND."@en .

:hasCuttingSpeedValue a owl:DatatypeProperty ;
	rdfs:subPropertyOf :hasSampledValue ;
        rdfs:range xsd:float ;
	rdfs:comment "Observed result for:  The speed difference (relative velocity) between the cutting mechanism and the surface of the workpiece it is operating on.. The units are MILLIMETER/SECOND."@en .

:ActualCuttingSpeed a owl:Class ;
	rdfs:subClassOf :CuttingSpeed ;
	rdfs:comment "The measured value of the data item type given by a sensor or encoder."@en .

:hasActualCuttingSpeedValue a owl:DatatypeProperty ;
	rdfs:subPropertyOf :hasCuttingSpeedValue ;
        rdfs:range xsd:float ;
	rdfs:comment "Observed result for: The measured value of the data item type given by a sensor or encoder."@en .

:CommandedCuttingSpeed a owl:Class ;
	rdfs:subClassOf :CuttingSpeed ;
	rdfs:comment "A value specified by the controller type component."@en .

:hasCommandedCuttingSpeedValue a owl:DatatypeProperty ;
	rdfs:subPropertyOf :hasCuttingSpeedValue ;
        rdfs:range xsd:float ;
	rdfs:comment "Observed result for: A value specified by the controller type component."@en .

:ProgrammedCuttingSpeed a owl:Class ;
	rdfs:subClassOf :CuttingSpeed ;
	rdfs:comment "The value of a signal or calculation specified by a logic or motion program or set by a switch."@en .

:hasProgrammedCuttingSpeedValue a owl:DatatypeProperty ;
	rdfs:subPropertyOf :hasCuttingSpeedValue ;
        rdfs:range xsd:float ;
	rdfs:comment "Observed result for: The value of a signal or calculation specified by a logic or motion program or set by a switch."@en .

[ rdf:type owl:AllDisjointClasses ;
        owl:members (
           :ActualCuttingSpeed
           :CommandedCuttingSpeed
           :ProgrammedCuttingSpeed
            )
        ] .

:Density a owl:Class ;
	rdfs:subClassOf :Sample ;
	rdfs:comment "The volumetric mass of a material per unit volume of that material.. The units are MILLIGRAM/CUBIC_MILLIMETER."@en .

:hasDensityValue a owl:DatatypeProperty ;
	rdfs:subPropertyOf :hasSampledValue ;
        rdfs:range xsd:float ;
	rdfs:comment "Observed result for: The volumetric mass of a material per unit volume of that material.. The units are MILLIGRAM/CUBIC_MILLIMETER."@en .

:DepositionAccelerationVolumetric a owl:Class ;
	rdfs:subClassOf :Sample ;
	rdfs:comment "The rate of change in spatial volume of material deposited in an additive manufacturing process.. The units are CUBIC_MILLIMETER/SECOND^2."@en .

:hasDepositionAccelerationVolumetricValue a owl:DatatypeProperty ;
	rdfs:subPropertyOf :hasSampledValue ;
        rdfs:range xsd:float ;
	rdfs:comment "Observed result for: The rate of change in spatial volume of material deposited in an additive manufacturing process.. The units are CUBIC_MILLIMETER/SECOND^2."@en .

:ActualDepositionAccelerationVolumetric a owl:Class ;
	rdfs:subClassOf :DepositionAccelerationVolumetric ;
	rdfs:comment "The measured value of the data item type given by a sensor or encoder."@en .

:hasActualDepositionAccelerationVolumetricValue a owl:DatatypeProperty ;
	rdfs:subPropertyOf :hasDepositionAccelerationVolumetricValue ;
        rdfs:range xsd:float ;
	rdfs:comment "Observed result for: The measured value of the data item type given by a sensor or encoder."@en .

:CommandedDepositionAccelerationVolumetric a owl:Class ;
	rdfs:subClassOf :DepositionAccelerationVolumetric ;
	rdfs:comment "A value specified by the controller type component."@en .

:hasCommandedDepositionAccelerationVolumetricValue a owl:DatatypeProperty ;
	rdfs:subPropertyOf :hasDepositionAccelerationVolumetricValue ;
        rdfs:range xsd:float ;
	rdfs:comment "Observed result for: A value specified by the controller type component."@en .

[ rdf:type owl:AllDisjointClasses ;
        owl:members (
           :ActualDepositionAccelerationVolumetric
           :CommandedDepositionAccelerationVolumetric
            )
        ] .

:DepositionDensity a owl:Class ;
	rdfs:subClassOf :Sample ;
	rdfs:comment "The density of the material deposited in an additive manufacturing process per unit of volume.. The units are MILLIGRAM/CUBIC_MILLIMETER."@en .

:hasDepositionDensityValue a owl:DatatypeProperty ;
	rdfs:subPropertyOf :hasSampledValue ;
        rdfs:range xsd:float ;
	rdfs:comment "Observed result for: The density of the material deposited in an additive manufacturing process per unit of volume.. The units are MILLIGRAM/CUBIC_MILLIMETER."@en .

:ActualDepositionDensity a owl:Class ;
	rdfs:subClassOf :DepositionDensity ;
	rdfs:comment "The measured value of the data item type given by a sensor or encoder."@en .

:hasActualDepositionDensityValue a owl:DatatypeProperty ;
	rdfs:subPropertyOf :hasDepositionDensityValue ;
        rdfs:range xsd:float ;
	rdfs:comment "Observed result for: The measured value of the data item type given by a sensor or encoder."@en .

:CommandedDepositionDensity a owl:Class ;
	rdfs:subClassOf :DepositionDensity ;
	rdfs:comment "A value specified by the controller type component."@en .

:hasCommandedDepositionDensityValue a owl:DatatypeProperty ;
	rdfs:subPropertyOf :hasDepositionDensityValue ;
        rdfs:range xsd:float ;
	rdfs:comment "Observed result for: A value specified by the controller type component."@en .

[ rdf:type owl:AllDisjointClasses ;
        owl:members (
           :ActualDepositionDensity
           :CommandedDepositionDensity
            )
        ] .

:DepositionMass a owl:Class ;
	rdfs:subClassOf :Sample ;
	rdfs:comment "The mass of the material deposited in an additive manufacturing process.. The units are MILLIGRAM."@en .

:hasDepositionMassValue a owl:DatatypeProperty ;
	rdfs:subPropertyOf :hasSampledValue ;
        rdfs:range xsd:float ;
	rdfs:comment "Observed result for: The mass of the material deposited in an additive manufacturing process.. The units are MILLIGRAM."@en .

:ActualDepositionMass a owl:Class ;
	rdfs:subClassOf :DepositionMass ;
	rdfs:comment "The measured value of the data item type given by a sensor or encoder."@en .

:hasActualDepositionMassValue a owl:DatatypeProperty ;
	rdfs:subPropertyOf :hasDepositionMassValue ;
        rdfs:range xsd:float ;
	rdfs:comment "Observed result for: The measured value of the data item type given by a sensor or encoder."@en .

:CommandedDepositionMass a owl:Class ;
	rdfs:subClassOf :DepositionMass ;
	rdfs:comment "A value specified by the controller type component."@en .

:hasCommandedDepositionMassValue a owl:DatatypeProperty ;
	rdfs:subPropertyOf :hasDepositionMassValue ;
        rdfs:range xsd:float ;
	rdfs:comment "Observed result for: A value specified by the controller type component."@en .

[ rdf:type owl:AllDisjointClasses ;
        owl:members (
           :ActualDepositionMass
           :CommandedDepositionMass
            )
        ] .

:DepositionRateVolumetric a owl:Class ;
	rdfs:subClassOf :Sample ;
	rdfs:comment "The rate at which a spatial volume of material is deposited in an additive manufacturing process.. The units are CUBIC_MILLIMETER/SECOND."@en .

:hasDepositionRateVolumetricValue a owl:DatatypeProperty ;
	rdfs:subPropertyOf :hasSampledValue ;
        rdfs:range xsd:float ;
	rdfs:comment "Observed result for: The rate at which a spatial volume of material is deposited in an additive manufacturing process.. The units are CUBIC_MILLIMETER/SECOND."@en .

:ActualDepositionRateVolumetric a owl:Class ;
	rdfs:subClassOf :DepositionRateVolumetric ;
	rdfs:comment "The measured value of the data item type given by a sensor or encoder."@en .

:hasActualDepositionRateVolumetricValue a owl:DatatypeProperty ;
	rdfs:subPropertyOf :hasDepositionRateVolumetricValue ;
        rdfs:range xsd:float ;
	rdfs:comment "Observed result for: The measured value of the data item type given by a sensor or encoder."@en .

:CommandedDepositionRateVolumetric a owl:Class ;
	rdfs:subClassOf :DepositionRateVolumetric ;
	rdfs:comment "A value specified by the controller type component."@en .

:hasCommandedDepositionRateVolumetricValue a owl:DatatypeProperty ;
	rdfs:subPropertyOf :hasDepositionRateVolumetricValue ;
        rdfs:range xsd:float ;
	rdfs:comment "Observed result for: A value specified by the controller type component."@en .

[ rdf:type owl:AllDisjointClasses ;
        owl:members (
           :ActualDepositionRateVolumetric
           :CommandedDepositionRateVolumetric
            )
        ] .

:DepositionVolume a owl:Class ;
	rdfs:subClassOf :Sample ;
	rdfs:comment "The spatial volume of material to be deposited in an additive manufacturing process.. The units are CUBIC_MILLIMETER."@en .

:hasDepositionVolumeValue a owl:DatatypeProperty ;
	rdfs:subPropertyOf :hasSampledValue ;
        rdfs:range xsd:float ;
	rdfs:comment "Observed result for: The spatial volume of material to be deposited in an additive manufacturing process.. The units are CUBIC_MILLIMETER."@en .

:ActualDepositionVolume a owl:Class ;
	rdfs:subClassOf :DepositionVolume ;
	rdfs:comment "The measured value of the data item type given by a sensor or encoder."@en .

:hasActualDepositionVolumeValue a owl:DatatypeProperty ;
	rdfs:subPropertyOf :hasDepositionVolumeValue ;
        rdfs:range xsd:float ;
	rdfs:comment "Observed result for: The measured value of the data item type given by a sensor or encoder."@en .

:CommandedDepositionVolume a owl:Class ;
	rdfs:subClassOf :DepositionVolume ;
	rdfs:comment "A value specified by the controller type component."@en .

:hasCommandedDepositionVolumeValue a owl:DatatypeProperty ;
	rdfs:subPropertyOf :hasDepositionVolumeValue ;
        rdfs:range xsd:float ;
	rdfs:comment "Observed result for: A value specified by the controller type component."@en .

[ rdf:type owl:AllDisjointClasses ;
        owl:members (
           :ActualDepositionVolume
           :CommandedDepositionVolume
            )
        ] .

:Displacement a owl:Class ;
	rdfs:subClassOf :Sample ;
	rdfs:comment "The measurement of the change in position of an object.. The units are MILLIMETER."@en .

:hasDisplacementValue a owl:DatatypeProperty ;
	rdfs:subPropertyOf :hasSampledValue ;
        rdfs:range xsd:float ;
	rdfs:comment "Observed result for: The measurement of the change in position of an object.. The units are MILLIMETER."@en .

:ElectricalEnergy a owl:Class ;
	rdfs:subClassOf :Sample ;
	rdfs:comment "The measurement of electrical energy consumption by a component.. The units are WATT_SECOND."@en .

:hasElectricalEnergyValue a owl:DatatypeProperty ;
	rdfs:subPropertyOf :hasSampledValue ;
        rdfs:range xsd:float ;
	rdfs:comment "Observed result for: The measurement of electrical energy consumption by a component.. The units are WATT_SECOND."@en .

:EquipmentTimer a owl:Class ;
	rdfs:subClassOf :Sample ;
	rdfs:comment "The measurement of the amount of time a piece of equipment or a sub-part of a piece of equipment has performed specific activities.. The units are SECOND."@en .

:hasEquipmentTimerValue a owl:DatatypeProperty ;
	rdfs:subPropertyOf :hasSampledValue ;
        rdfs:range xsd:float ;
	rdfs:comment "Observed result for: The measurement of the amount of time a piece of equipment or a sub-part of a piece of equipment has performed specific activities.. The units are SECOND."@en .

:LoadedEquipmentTimer a owl:Class ;
	rdfs:subClassOf :EquipmentTimer ;
	rdfs:comment "Subparts of a piece of equipment are under load."@en .

:hasLoadedEquipmentTimerValue a owl:DatatypeProperty ;
	rdfs:subPropertyOf :hasEquipmentTimerValue ;
        rdfs:range xsd:float ;
	rdfs:comment "Observed result for: Subparts of a piece of equipment are under load."@en .

:WorkingEquipmentTimer a owl:Class ;
	rdfs:subClassOf :EquipmentTimer ;
	rdfs:comment "A piece of equipment performing any activity, the equipment is active and performing a function under load or not."@en .

:hasWorkingEquipmentTimerValue a owl:DatatypeProperty ;
	rdfs:subPropertyOf :hasEquipmentTimerValue ;
        rdfs:range xsd:float ;
	rdfs:comment "Observed result for: A piece of equipment performing any activity, the equipment is active and performing a function under load or not."@en .

:OperatingEquipmentTimer a owl:Class ;
	rdfs:subClassOf :EquipmentTimer ;
	rdfs:comment "A piece of equipment are powered or performing any activity."@en .

:hasOperatingEquipmentTimerValue a owl:DatatypeProperty ;
	rdfs:subPropertyOf :hasEquipmentTimerValue ;
        rdfs:range xsd:float ;
	rdfs:comment "Observed result for: A piece of equipment are powered or performing any activity."@en .

:PoweredEquipmentTimer a owl:Class ;
	rdfs:subClassOf :EquipmentTimer ;
	rdfs:comment "Primary  power is  applied  to the  piece  of  equipment and,  as  a minimum, the controller or logic portion of the piece of equipment is powered and functioning or components that are required to remain on are powered."@en .

:hasPoweredEquipmentTimerValue a owl:DatatypeProperty ;
	rdfs:subPropertyOf :hasEquipmentTimerValue ;
        rdfs:range xsd:float ;
	rdfs:comment "Observed result for: Primary  power is  applied  to the  piece  of  equipment and,  as  a minimum, the controller or logic portion of the piece of equipment is powered and functioning or components that are required to remain on are powered."@en .

:DelayEquipmentTimer a owl:Class ;
	rdfs:subClassOf :EquipmentTimer ;
	rdfs:comment "A piece of equipment waiting for an event or an action to occur."@en .

:hasDelayEquipmentTimerValue a owl:DatatypeProperty ;
	rdfs:subPropertyOf :hasEquipmentTimerValue ;
        rdfs:range xsd:float ;
	rdfs:comment "Observed result for: A piece of equipment waiting for an event or an action to occur."@en .

[ rdf:type owl:AllDisjointClasses ;
        owl:members (
           :LoadedEquipmentTimer
           :WorkingEquipmentTimer
           :OperatingEquipmentTimer
           :PoweredEquipmentTimer
           :DelayEquipmentTimer
            )
        ] .

:FillLevel a owl:Class ;
	rdfs:subClassOf :Sample ;
	rdfs:comment "The measurement of the amount of a substance remaining compared to the planned maximum amount of that substance.. The units are PERCENT."@en .

:hasFillLevelValue a owl:DatatypeProperty ;
	rdfs:subPropertyOf :hasSampledValue ;
        rdfs:range xsd:float ;
	rdfs:comment "Observed result for: The measurement of the amount of a substance remaining compared to the planned maximum amount of that substance.. The units are PERCENT."@en .

:Flow a owl:Class ;
	rdfs:subClassOf :Sample ;
	rdfs:comment "The measurement of the rate of flow of a fluid.. The units are LITER/SECOND."@en .

:hasFlowValue a owl:DatatypeProperty ;
	rdfs:subPropertyOf :hasSampledValue ;
        rdfs:range xsd:float ;
	rdfs:comment "Observed result for: The measurement of the rate of flow of a fluid.. The units are LITER/SECOND."@en .

:Frequency a owl:Class ;
	rdfs:subClassOf :Sample ;
	rdfs:comment "The measurement of the number of occurrences of a repeating event per unit time.. The units are HERTZ."@en .

:hasFrequencyValue a owl:DatatypeProperty ;
	rdfs:subPropertyOf :hasSampledValue ;
        rdfs:range xsd:float ;
	rdfs:comment "Observed result for: The measurement of the number of occurrences of a repeating event per unit time.. The units are HERTZ."@en .

:GlobalPosition a owl:Class ;
	rdfs:subClassOf :Sample ;
	rdfs:comment "DEPRECATED in Version 1.1. The units are ."@en .

:hasGlobalPositionValue a owl:DatatypeProperty ;
	rdfs:subPropertyOf :hasSampledValue ;
        rdfs:range xsd:float ;
	rdfs:comment "Observed result for: DEPRECATED in Version 1.1. The units are ."@en .

:Length a owl:Class ;
	rdfs:subClassOf :Sample ;
	rdfs:comment "The measurement of the length of an object.. The units are MILLIMETER."@en .

:hasLengthValue a owl:DatatypeProperty ;
	rdfs:subPropertyOf :hasSampledValue ;
        rdfs:range xsd:float ;
	rdfs:comment "Observed result for: The measurement of the length of an object.. The units are MILLIMETER."@en .

:StandardLength a owl:Class ;
	rdfs:subClassOf :Length ;
	rdfs:comment "The standard or original length of an object."@en .

:hasStandardLengthValue a owl:DatatypeProperty ;
	rdfs:subPropertyOf :hasLengthValue ;
        rdfs:range xsd:float ;
	rdfs:comment "Observed result for: The standard or original length of an object."@en .

:RemainingLength a owl:Class ;
	rdfs:subClassOf :Length ;
	rdfs:comment "Remaining measure of an object or an action."@en .

:hasRemainingLengthValue a owl:DatatypeProperty ;
	rdfs:subPropertyOf :hasLengthValue ;
        rdfs:range xsd:float ;
	rdfs:comment "Observed result for: Remaining measure of an object or an action."@en .

:UseableLength a owl:Class ;
	rdfs:subClassOf :Length ;
	rdfs:comment "The remaining useable length of an object."@en .

:hasUseableLengthValue a owl:DatatypeProperty ;
	rdfs:subPropertyOf :hasLengthValue ;
        rdfs:range xsd:float ;
	rdfs:comment "Observed result for: The remaining useable length of an object."@en .

[ rdf:type owl:AllDisjointClasses ;
        owl:members (
           :StandardLength
           :RemainingLength
           :UseableLength
            )
        ] .

:Level a owl:Class ;
	rdfs:subClassOf :Sample ;
	rdfs:comment "DEPRECATED in Version 1.2.  See filllevel sample. The units are ."@en .

:hasLevelValue a owl:DatatypeProperty ;
	rdfs:subPropertyOf :hasSampledValue ;
        rdfs:range xsd:float ;
	rdfs:comment "Observed result for: DEPRECATED in Version 1.2.  See filllevel sample. The units are ."@en .

:LinearForce a owl:Class ;
	rdfs:subClassOf :Sample ;
	rdfs:comment "The measurement of the push or pull introduced by an actuator or exerted on an object.. The units are NEWTON."@en .

:hasLinearForceValue a owl:DatatypeProperty ;
	rdfs:subPropertyOf :hasSampledValue ;
        rdfs:range xsd:float ;
	rdfs:comment "Observed result for: The measurement of the push or pull introduced by an actuator or exerted on an object.. The units are NEWTON."@en .

:Load a owl:Class ;
	rdfs:subClassOf :Sample ;
	rdfs:comment "The measurement of the actual versus the standard rating of a piece of equipment.. The units are PERCENT."@en .

:hasLoadValue a owl:DatatypeProperty ;
	rdfs:subPropertyOf :hasSampledValue ;
        rdfs:range xsd:float ;
	rdfs:comment "Observed result for: The measurement of the actual versus the standard rating of a piece of equipment.. The units are PERCENT."@en .

:Mass a owl:Class ;
	rdfs:subClassOf :Sample ;
	rdfs:comment "The measurement of the mass of an object(s) or an amount of material.. The units are KILOGRAM."@en .

:hasMassValue a owl:DatatypeProperty ;
	rdfs:subPropertyOf :hasSampledValue ;
        rdfs:range xsd:float ;
	rdfs:comment "Observed result for: The measurement of the mass of an object(s) or an amount of material.. The units are KILOGRAM."@en .

:PathFeedrate a owl:Class ;
	rdfs:subClassOf :Sample ;
	rdfs:comment "The measurement of the feedrate for the axes, or a single axis, associated with a path component-a vector.. The units are MILLIMETER/SECOND."@en .

:hasPathFeedrateValue a owl:DatatypeProperty ;
	rdfs:subPropertyOf :hasSampledValue ;
        rdfs:range xsd:float ;
	rdfs:comment "Observed result for: The measurement of the feedrate for the axes, or a single axis, associated with a path component-a vector.. The units are MILLIMETER/SECOND."@en .

:ActualPathFeedrate a owl:Class ;
	rdfs:subClassOf :PathFeedrate ;
	rdfs:comment "The measured value of the data item type given by a sensor or encoder."@en .

:hasActualPathFeedrateValue a owl:DatatypeProperty ;
	rdfs:subPropertyOf :hasPathFeedrateValue ;
        rdfs:range xsd:float ;
	rdfs:comment "Observed result for: The measured value of the data item type given by a sensor or encoder."@en .

:CommandedPathFeedrate a owl:Class ;
	rdfs:subClassOf :PathFeedrate ;
	rdfs:comment "A value specified by the controller type component."@en .

:hasCommandedPathFeedrateValue a owl:DatatypeProperty ;
	rdfs:subPropertyOf :hasPathFeedrateValue ;
        rdfs:range xsd:float ;
	rdfs:comment "Observed result for: A value specified by the controller type component."@en .

:JogPathFeedrate a owl:Class ;
	rdfs:subClassOf :PathFeedrate ;
	rdfs:comment "The feedrate specified by a logic or motion program, by a pre-set value, or set by a switch as the feedrate for the axes. "@en .

:hasJogPathFeedrateValue a owl:DatatypeProperty ;
	rdfs:subPropertyOf :hasPathFeedrateValue ;
        rdfs:range xsd:float ;
	rdfs:comment "Observed result for: The feedrate specified by a logic or motion program, by a pre-set value, or set by a switch as the feedrate for the axes. "@en .

:ProgrammedPathFeedrate a owl:Class ;
	rdfs:subClassOf :PathFeedrate ;
	rdfs:comment "The value of a signal or calculation specified by a logic or motion program or set by a switch."@en .

:hasProgrammedPathFeedrateValue a owl:DatatypeProperty ;
	rdfs:subPropertyOf :hasPathFeedrateValue ;
        rdfs:range xsd:float ;
	rdfs:comment "Observed result for: The value of a signal or calculation specified by a logic or motion program or set by a switch."@en .

:RapidPathFeedrate a owl:Class ;
	rdfs:subClassOf :PathFeedrate ;
	rdfs:comment "The value of a signal or calculation issued to adjust the feedrate of a component or composition that is operating in a rapid positioning mode."@en .

:hasRapidPathFeedrateValue a owl:DatatypeProperty ;
	rdfs:subPropertyOf :hasPathFeedrateValue ;
        rdfs:range xsd:float ;
	rdfs:comment "Observed result for: The value of a signal or calculation issued to adjust the feedrate of a component or composition that is operating in a rapid positioning mode."@en .

:OverridePathFeedrate a owl:Class ;
	rdfs:subClassOf :PathFeedrate ;
	rdfs:comment "DEPRECATED: The operators overridden value."@en .

:hasOverridePathFeedrateValue a owl:DatatypeProperty ;
	rdfs:subPropertyOf :hasPathFeedrateValue ;
        rdfs:range xsd:float ;
	rdfs:comment "Observed result for: DEPRECATED: The operators overridden value."@en .

[ rdf:type owl:AllDisjointClasses ;
        owl:members (
           :ActualPathFeedrate
           :CommandedPathFeedrate
           :JogPathFeedrate
           :ProgrammedPathFeedrate
           :RapidPathFeedrate
           :OverridePathFeedrate
            )
        ] .

:PathFeedratePerRevolution a owl:Class ;
	rdfs:subClassOf :Sample ;
	rdfs:comment "The feedrate for the axes, or a single axis.. The units are MILLIMETER/REVOLUTION."@en .

:hasPathFeedratePerRevolutionValue a owl:DatatypeProperty ;
	rdfs:subPropertyOf :hasSampledValue ;
        rdfs:range xsd:float ;
	rdfs:comment "Observed result for: The feedrate for the axes, or a single axis.. The units are MILLIMETER/REVOLUTION."@en .

:ActualPathFeedratePerRevolution a owl:Class ;
	rdfs:subClassOf :PathFeedratePerRevolution ;
	rdfs:comment "The measured value of the data item type given by a sensor or encoder."@en .

:hasActualPathFeedratePerRevolutionValue a owl:DatatypeProperty ;
	rdfs:subPropertyOf :hasPathFeedratePerRevolutionValue ;
        rdfs:range xsd:float ;
	rdfs:comment "Observed result for: The measured value of the data item type given by a sensor or encoder."@en .

:CommandedPathFeedratePerRevolution a owl:Class ;
	rdfs:subClassOf :PathFeedratePerRevolution ;
	rdfs:comment "A value specified by the controller type component."@en .

:hasCommandedPathFeedratePerRevolutionValue a owl:DatatypeProperty ;
	rdfs:subPropertyOf :hasPathFeedratePerRevolutionValue ;
        rdfs:range xsd:float ;
	rdfs:comment "Observed result for: A value specified by the controller type component."@en .

:ProgrammedPathFeedratePerRevolution a owl:Class ;
	rdfs:subClassOf :PathFeedratePerRevolution ;
	rdfs:comment "The value of a signal or calculation specified by a logic or motion program or set by a switch."@en .

:hasProgrammedPathFeedratePerRevolutionValue a owl:DatatypeProperty ;
	rdfs:subPropertyOf :hasPathFeedratePerRevolutionValue ;
        rdfs:range xsd:float ;
	rdfs:comment "Observed result for: The value of a signal or calculation specified by a logic or motion program or set by a switch."@en .

[ rdf:type owl:AllDisjointClasses ;
        owl:members (
           :ActualPathFeedratePerRevolution
           :CommandedPathFeedratePerRevolution
           :ProgrammedPathFeedratePerRevolution
            )
        ] .

:PathPosition a owl:Class ;
	rdfs:subClassOf :Sample ;
	rdfs:comment "A measured or calculated position of a control point associated with a controller element, or path element if provided, of a piece of equipment.. The units are MILLIMETER_3D."@en .

:hasPathPositionValue a owl:DatatypeProperty ;
	rdfs:subPropertyOf :hasSampledValue ;
        rdfs:range xsd:float ;
	rdfs:comment "Observed result for: A measured or calculated position of a control point associated with a controller element, or path element if provided, of a piece of equipment.. The units are MILLIMETER_3D."@en .

:ActualPathPosition a owl:Class ;
	rdfs:subClassOf :PathPosition ;
	rdfs:comment "The measured value of the data item type given by a sensor or encoder."@en .

:hasActualPathPositionValue a owl:DatatypeProperty ;
	rdfs:subPropertyOf :hasPathPositionValue ;
        rdfs:range xsd:float ;
	rdfs:comment "Observed result for: The measured value of the data item type given by a sensor or encoder."@en .

:CommandedPathPosition a owl:Class ;
	rdfs:subClassOf :PathPosition ;
	rdfs:comment "A value specified by the controller type component."@en .

:hasCommandedPathPositionValue a owl:DatatypeProperty ;
	rdfs:subPropertyOf :hasPathPositionValue ;
        rdfs:range xsd:float ;
	rdfs:comment "Observed result for: A value specified by the controller type component."@en .

:TargetPathPosition a owl:Class ;
	rdfs:subClassOf :PathPosition ;
	rdfs:comment "The desired measure or count for a data item value."@en .

:hasTargetPathPositionValue a owl:DatatypeProperty ;
	rdfs:subPropertyOf :hasPathPositionValue ;
        rdfs:range xsd:float ;
	rdfs:comment "Observed result for: The desired measure or count for a data item value."@en .

:ProbePathPosition a owl:Class ;
	rdfs:subClassOf :PathPosition ;
	rdfs:comment "The position provided by a measurement probe."@en .

:hasProbePathPositionValue a owl:DatatypeProperty ;
	rdfs:subPropertyOf :hasPathPositionValue ;
        rdfs:range xsd:float ;
	rdfs:comment "Observed result for: The position provided by a measurement probe."@en .

[ rdf:type owl:AllDisjointClasses ;
        owl:members (
           :ActualPathPosition
           :CommandedPathPosition
           :TargetPathPosition
           :ProbePathPosition
            )
        ] .

:PH a owl:Class ;
	rdfs:subClassOf :Sample ;
	rdfs:comment "A measure of the acidity or alkalinity of a solution.. The units are PH."@en .

:hasPHValue a owl:DatatypeProperty ;
	rdfs:subPropertyOf :hasSampledValue ;
        rdfs:range xsd:float ;
	rdfs:comment "Observed result for: A measure of the acidity or alkalinity of a solution.. The units are PH."@en .

:Position a owl:Class ;
	rdfs:subClassOf :Sample ;
	rdfs:comment "A measured or calculated position of a component element as reported by a piece of equipment.. The units are MILLIMETER."@en .

:hasPositionValue a owl:DatatypeProperty ;
	rdfs:subPropertyOf :hasSampledValue ;
        rdfs:range xsd:float ;
	rdfs:comment "Observed result for: A measured or calculated position of a component element as reported by a piece of equipment.. The units are MILLIMETER."@en .

:ActualPosition a owl:Class ;
	rdfs:subClassOf :Position ;
	rdfs:comment "The measured value of the data item type given by a sensor or encoder."@en .

:hasActualPositionValue a owl:DatatypeProperty ;
	rdfs:subPropertyOf :hasPositionValue ;
        rdfs:range xsd:float ;
	rdfs:comment "Observed result for: The measured value of the data item type given by a sensor or encoder."@en .

:CommandedPosition a owl:Class ;
	rdfs:subClassOf :Position ;
	rdfs:comment "A value specified by the controller type component."@en .

:hasCommandedPositionValue a owl:DatatypeProperty ;
	rdfs:subPropertyOf :hasPositionValue ;
        rdfs:range xsd:float ;
	rdfs:comment "Observed result for: A value specified by the controller type component."@en .

:ProgrammedPosition a owl:Class ;
	rdfs:subClassOf :Position ;
	rdfs:comment "The value of a signal or calculation specified by a logic or motion program or set by a switch."@en .

:hasProgrammedPositionValue a owl:DatatypeProperty ;
	rdfs:subPropertyOf :hasPositionValue ;
        rdfs:range xsd:float ;
	rdfs:comment "Observed result for: The value of a signal or calculation specified by a logic or motion program or set by a switch."@en .

:TargetPosition a owl:Class ;
	rdfs:subClassOf :Position ;
	rdfs:comment "The desired measure or count for a data item value."@en .

:hasTargetPositionValue a owl:DatatypeProperty ;
	rdfs:subPropertyOf :hasPositionValue ;
        rdfs:range xsd:float ;
	rdfs:comment "Observed result for: The desired measure or count for a data item value."@en .

[ rdf:type owl:AllDisjointClasses ;
        owl:members (
           :ActualPosition
           :CommandedPosition
           :ProgrammedPosition
           :TargetPosition
            )
        ] .

:PowerFactor a owl:Class ;
	rdfs:subClassOf :Sample ;
	rdfs:comment "The measurement of the ratio of real power flowing to a load to the apparent power in that AC circuit.. The units are PERCENT."@en .

:hasPowerFactorValue a owl:DatatypeProperty ;
	rdfs:subPropertyOf :hasSampledValue ;
        rdfs:range xsd:float ;
	rdfs:comment "Observed result for: The measurement of the ratio of real power flowing to a load to the apparent power in that AC circuit.. The units are PERCENT."@en .

:Pressure a owl:Class ;
	rdfs:subClassOf :Sample ;
	rdfs:comment "The measurement of force per unit area exerted by a gas or liquid.. The units are PASCAL."@en .

:hasPressureValue a owl:DatatypeProperty ;
	rdfs:subPropertyOf :hasSampledValue ;
        rdfs:range xsd:float ;
	rdfs:comment "Observed result for: The measurement of force per unit area exerted by a gas or liquid.. The units are PASCAL."@en .

:ProcessTimer a owl:Class ;
	rdfs:subClassOf :Sample ;
	rdfs:comment "The measurement of the amount of time a piece of equipment has performed different types of activities associated with the process being performed at that piece of equipment.. The units are SECOND."@en .

:hasProcessTimerValue a owl:DatatypeProperty ;
	rdfs:subPropertyOf :hasSampledValue ;
        rdfs:range xsd:float ;
	rdfs:comment "Observed result for: The measurement of the amount of time a piece of equipment has performed different types of activities associated with the process being performed at that piece of equipment.. The units are SECOND."@en .

:ProcessProcessTimer a owl:Class ;
	rdfs:subClassOf :ProcessTimer ;
	rdfs:comment "The measurement of the time from the beginning of production of a part or product on a piece of equipment until the time that production is complete for that part or product on that piece of equipment.  This includes the time that the piece of equipment is running, producing parts or products, or in the process of producing parts."@en .

:hasProcessProcessTimerValue a owl:DatatypeProperty ;
	rdfs:subPropertyOf :hasProcessTimerValue ;
        rdfs:range xsd:float ;
	rdfs:comment "Observed result for: The measurement of the time from the beginning of production of a part or product on a piece of equipment until the time that production is complete for that part or product on that piece of equipment.  This includes the time that the piece of equipment is running, producing parts or products, or in the process of producing parts."@en .

:DelayProcessTimer a owl:Class ;
	rdfs:subClassOf :ProcessTimer ;
	rdfs:comment "A piece of equipment waiting for an event or an action to occur."@en .

:hasDelayProcessTimerValue a owl:DatatypeProperty ;
	rdfs:subPropertyOf :hasProcessTimerValue ;
        rdfs:range xsd:float ;
	rdfs:comment "Observed result for: A piece of equipment waiting for an event or an action to occur."@en .

[ rdf:type owl:AllDisjointClasses ;
        owl:members (
           :ProcessProcessTimer
           :DelayProcessTimer
            )
        ] .

:Resistance a owl:Class ;
	rdfs:subClassOf :Sample ;
	rdfs:comment "The measurement of the degree to which a substance opposes the passage of an electric current.. The units are OHM."@en .

:hasResistanceValue a owl:DatatypeProperty ;
	rdfs:subPropertyOf :hasSampledValue ;
        rdfs:range xsd:float ;
	rdfs:comment "Observed result for: The measurement of the degree to which a substance opposes the passage of an electric current.. The units are OHM."@en .

:RotaryVelocity a owl:Class ;
	rdfs:subClassOf :Sample ;
	rdfs:comment "The measurement of the rotational speed of a rotary axis.. The units are REVOLUTION/MINUTE."@en .

:hasRotaryVelocityValue a owl:DatatypeProperty ;
	rdfs:subPropertyOf :hasSampledValue ;
        rdfs:range xsd:float ;
	rdfs:comment "Observed result for: The measurement of the rotational speed of a rotary axis.. The units are REVOLUTION/MINUTE."@en .

:ActualRotaryVelocity a owl:Class ;
	rdfs:subClassOf :RotaryVelocity ;
	rdfs:comment "The measured value of the data item type given by a sensor or encoder."@en .

:hasActualRotaryVelocityValue a owl:DatatypeProperty ;
	rdfs:subPropertyOf :hasRotaryVelocityValue ;
        rdfs:range xsd:float ;
	rdfs:comment "Observed result for: The measured value of the data item type given by a sensor or encoder."@en .

:CommandedRotaryVelocity a owl:Class ;
	rdfs:subClassOf :RotaryVelocity ;
	rdfs:comment "A value specified by the controller type component."@en .

:hasCommandedRotaryVelocityValue a owl:DatatypeProperty ;
	rdfs:subPropertyOf :hasRotaryVelocityValue ;
        rdfs:range xsd:float ;
	rdfs:comment "Observed result for: A value specified by the controller type component."@en .

:ProgrammedRotaryVelocity a owl:Class ;
	rdfs:subClassOf :RotaryVelocity ;
	rdfs:comment "The value of a signal or calculation specified by a logic or motion program or set by a switch."@en .

:hasProgrammedRotaryVelocityValue a owl:DatatypeProperty ;
	rdfs:subPropertyOf :hasRotaryVelocityValue ;
        rdfs:range xsd:float ;
	rdfs:comment "Observed result for: The value of a signal or calculation specified by a logic or motion program or set by a switch."@en .

:OverrideRotaryVelocity a owl:Class ;
	rdfs:subClassOf :RotaryVelocity ;
	rdfs:comment "DEPRECATED: The operators overridden value."@en .

:hasOverrideRotaryVelocityValue a owl:DatatypeProperty ;
	rdfs:subPropertyOf :hasRotaryVelocityValue ;
        rdfs:range xsd:float ;
	rdfs:comment "Observed result for: DEPRECATED: The operators overridden value."@en .

[ rdf:type owl:AllDisjointClasses ;
        owl:members (
           :ActualRotaryVelocity
           :CommandedRotaryVelocity
           :ProgrammedRotaryVelocity
           :OverrideRotaryVelocity
            )
        ] .

:SoundLevel a owl:Class ;
	rdfs:subClassOf :Sample ;
	rdfs:comment "The measurement of a sound level or sound pressure level relative to atmospheric pressure.. The units are DECIBEL."@en .

:hasSoundLevelValue a owl:DatatypeProperty ;
	rdfs:subPropertyOf :hasSampledValue ;
        rdfs:range xsd:float ;
	rdfs:comment "Observed result for: The measurement of a sound level or sound pressure level relative to atmospheric pressure.. The units are DECIBEL."@en .

:NoScaleSoundLevel a owl:Class ;
	rdfs:subClassOf :SoundLevel ;
	rdfs:comment "No weighting factor on the frequency scale"@en .

:hasNoScaleSoundLevelValue a owl:DatatypeProperty ;
	rdfs:subPropertyOf :hasSoundLevelValue ;
        rdfs:range xsd:float ;
	rdfs:comment "Observed result for: No weighting factor on the frequency scale"@en .

:AScaleSoundLevel a owl:Class ;
	rdfs:subClassOf :SoundLevel ;
	rdfs:comment "A Scale weighting factor.   This is the default weighting factor if no factor is specified"@en .

:hasAScaleSoundLevelValue a owl:DatatypeProperty ;
	rdfs:subPropertyOf :hasSoundLevelValue ;
        rdfs:range xsd:float ;
	rdfs:comment "Observed result for: A Scale weighting factor.   This is the default weighting factor if no factor is specified"@en .

:BScaleSoundLevel a owl:Class ;
	rdfs:subClassOf :SoundLevel ;
	rdfs:comment "B Scale weighting factor"@en .

:hasBScaleSoundLevelValue a owl:DatatypeProperty ;
	rdfs:subPropertyOf :hasSoundLevelValue ;
        rdfs:range xsd:float ;
	rdfs:comment "Observed result for: B Scale weighting factor"@en .

:CScaleSoundLevel a owl:Class ;
	rdfs:subClassOf :SoundLevel ;
	rdfs:comment "C Scale weighting factor"@en .

:hasCScaleSoundLevelValue a owl:DatatypeProperty ;
	rdfs:subPropertyOf :hasSoundLevelValue ;
        rdfs:range xsd:float ;
	rdfs:comment "Observed result for: C Scale weighting factor"@en .

:DScaleSoundLevel a owl:Class ;
	rdfs:subClassOf :SoundLevel ;
	rdfs:comment "D Scale weighting factor"@en .

:hasDScaleSoundLevelValue a owl:DatatypeProperty ;
	rdfs:subPropertyOf :hasSoundLevelValue ;
        rdfs:range xsd:float ;
	rdfs:comment "Observed result for: D Scale weighting factor"@en .

[ rdf:type owl:AllDisjointClasses ;
        owl:members (
           :NoScaleSoundLevel
           :AScaleSoundLevel
           :BScaleSoundLevel
           :CScaleSoundLevel
           :DScaleSoundLevel
            )
        ] .

:SpindleSpeed a owl:Class ;
	rdfs:subClassOf :Sample ;
	rdfs:comment "DEPRECATED in Version 1.2.  Replaced by rotaryvelocity sample. The units are REVOLUTION/MINUTE."@en .

:hasSpindleSpeedValue a owl:DatatypeProperty ;
	rdfs:subPropertyOf :hasSampledValue ;
        rdfs:range xsd:float ;
	rdfs:comment "Observed result for: DEPRECATED in Version 1.2.  Replaced by rotaryvelocity sample. The units are REVOLUTION/MINUTE."@en .

:ActualSpindleSpeed a owl:Class ;
	rdfs:subClassOf :SpindleSpeed ;
	rdfs:comment "The measured value of the data item type given by a sensor or encoder."@en .

:hasActualSpindleSpeedValue a owl:DatatypeProperty ;
	rdfs:subPropertyOf :hasSpindleSpeedValue ;
        rdfs:range xsd:float ;
	rdfs:comment "Observed result for: The measured value of the data item type given by a sensor or encoder."@en .

:CommandedSpindleSpeed a owl:Class ;
	rdfs:subClassOf :SpindleSpeed ;
	rdfs:comment "A value specified by the controller type component."@en .

:hasCommandedSpindleSpeedValue a owl:DatatypeProperty ;
	rdfs:subPropertyOf :hasSpindleSpeedValue ;
        rdfs:range xsd:float ;
	rdfs:comment "Observed result for: A value specified by the controller type component."@en .

:OverrideSpindleSpeed a owl:Class ;
	rdfs:subClassOf :SpindleSpeed ;
	rdfs:comment "DEPRECATED: The operators overridden value."@en .

:hasOverrideSpindleSpeedValue a owl:DatatypeProperty ;
	rdfs:subPropertyOf :hasSpindleSpeedValue ;
        rdfs:range xsd:float ;
	rdfs:comment "Observed result for: DEPRECATED: The operators overridden value."@en .

[ rdf:type owl:AllDisjointClasses ;
        owl:members (
           :ActualSpindleSpeed
           :CommandedSpindleSpeed
           :OverrideSpindleSpeed
            )
        ] .

:Strain a owl:Class ;
	rdfs:subClassOf :Sample ;
	rdfs:comment "The measurement of the amount of deformation per unit length of an object when a load is applied.. The units are PERCENT."@en .

:hasStrainValue a owl:DatatypeProperty ;
	rdfs:subPropertyOf :hasSampledValue ;
        rdfs:range xsd:float ;
	rdfs:comment "Observed result for: The measurement of the amount of deformation per unit length of an object when a load is applied.. The units are PERCENT."@en .

:Temperature a owl:Class ;
	rdfs:subClassOf :Sample ;
	rdfs:comment "The measurement of temperature.. The units are CELSIUS."@en .

:hasTemperatureValue a owl:DatatypeProperty ;
	rdfs:subPropertyOf :hasSampledValue ;
        rdfs:range xsd:float ;
	rdfs:comment "Observed result for: The measurement of temperature.. The units are CELSIUS."@en .

:Tension a owl:Class ;
	rdfs:subClassOf :Sample ;
	rdfs:comment "The measurement of a force that stretches or elongates an object.. The units are NEWTON."@en .

:hasTensionValue a owl:DatatypeProperty ;
	rdfs:subPropertyOf :hasSampledValue ;
        rdfs:range xsd:float ;
	rdfs:comment "Observed result for: The measurement of a force that stretches or elongates an object.. The units are NEWTON."@en .

:Tilt a owl:Class ;
	rdfs:subClassOf :Sample ;
	rdfs:comment "The measurement of angular displacement. . The units are MICRO_RADIAN."@en .

:hasTiltValue a owl:DatatypeProperty ;
	rdfs:subPropertyOf :hasSampledValue ;
        rdfs:range xsd:float ;
	rdfs:comment "Observed result for: The measurement of angular displacement. . The units are MICRO_RADIAN."@en .

:Torque a owl:Class ;
	rdfs:subClassOf :Sample ;
	rdfs:comment "The measurement of the turning force exerted on an object or by an object.. The units are NEWTON_METER."@en .

:hasTorqueValue a owl:DatatypeProperty ;
	rdfs:subPropertyOf :hasSampledValue ;
        rdfs:range xsd:float ;
	rdfs:comment "Observed result for: The measurement of the turning force exerted on an object or by an object.. The units are NEWTON_METER."@en .

:Velocity a owl:Class ;
	rdfs:subClassOf :Sample ;
	rdfs:comment "The measurement of the rate of change of position of a component.. The units are MILLIMETER/SECOND."@en .

:hasVelocityValue a owl:DatatypeProperty ;
	rdfs:subPropertyOf :hasSampledValue ;
        rdfs:range xsd:float ;
	rdfs:comment "Observed result for: The measurement of the rate of change of position of a component.. The units are MILLIMETER/SECOND."@en .

:Viscosity a owl:Class ;
	rdfs:subClassOf :Sample ;
	rdfs:comment "The measurement of a fluids resistance to flow.. The units are PASCAL_SECOND."@en .

:hasViscosityValue a owl:DatatypeProperty ;
	rdfs:subPropertyOf :hasSampledValue ;
        rdfs:range xsd:float ;
	rdfs:comment "Observed result for: The measurement of a fluids resistance to flow.. The units are PASCAL_SECOND."@en .

:Voltage a owl:Class ;
	rdfs:subClassOf :Sample ;
	rdfs:comment "The measurement of electrical potential between two points.. The units are VOLT."@en .

:hasVoltageValue a owl:DatatypeProperty ;
	rdfs:subPropertyOf :hasSampledValue ;
        rdfs:range xsd:float ;
	rdfs:comment "Observed result for: The measurement of electrical potential between two points.. The units are VOLT."@en .

:AlternatingVoltage a owl:Class ;
	rdfs:subClassOf :Voltage ;
	rdfs:comment "The measurement of alternating voltage or current.   If not specified further in statistic, defaults to RMS voltage. "@en .

:hasAlternatingVoltageValue a owl:DatatypeProperty ;
	rdfs:subPropertyOf :hasVoltageValue ;
        rdfs:range xsd:float ;
	rdfs:comment "Observed result for: The measurement of alternating voltage or current.   If not specified further in statistic, defaults to RMS voltage. "@en .

:DirectVoltage a owl:Class ;
	rdfs:subClassOf :Voltage ;
	rdfs:comment "The measurement of DC current or voltage."@en .

:hasDirectVoltageValue a owl:DatatypeProperty ;
	rdfs:subPropertyOf :hasVoltageValue ;
        rdfs:range xsd:float ;
	rdfs:comment "Observed result for: The measurement of DC current or voltage."@en .

:ActualVoltage a owl:Class ;
	rdfs:subClassOf :Voltage ;
	rdfs:comment "The measured value of the data item type given by a sensor or encoder."@en .

:hasActualVoltageValue a owl:DatatypeProperty ;
	rdfs:subPropertyOf :hasVoltageValue ;
        rdfs:range xsd:float ;
	rdfs:comment "Observed result for: The measured value of the data item type given by a sensor or encoder."@en .

:TargetVoltage a owl:Class ;
	rdfs:subClassOf :Voltage ;
	rdfs:comment "The desired measure or count for a data item value."@en .

:hasTargetVoltageValue a owl:DatatypeProperty ;
	rdfs:subPropertyOf :hasVoltageValue ;
        rdfs:range xsd:float ;
	rdfs:comment "Observed result for: The desired measure or count for a data item value."@en .

[ rdf:type owl:AllDisjointClasses ;
        owl:members (
           :AlternatingVoltage
           :DirectVoltage
           :ActualVoltage
           :TargetVoltage
            )
        ] .

:VoltAmpere a owl:Class ;
	rdfs:subClassOf :Sample ;
	rdfs:comment "The measurement of the apparent power in an electrical circuit, equal to the product of root-mean-square (RMS) voltage and RMS current (commonly referred to as VA).. The units are VOLT_AMPERE."@en .

:hasVoltAmpereValue a owl:DatatypeProperty ;
	rdfs:subPropertyOf :hasSampledValue ;
        rdfs:range xsd:float ;
	rdfs:comment "Observed result for: The measurement of the apparent power in an electrical circuit, equal to the product of root-mean-square (RMS) voltage and RMS current (commonly referred to as VA).. The units are VOLT_AMPERE."@en .

:VoltAmpereReactive a owl:Class ;
	rdfs:subClassOf :Sample ;
	rdfs:comment "The measurement of reactive power in an AC electrical circuit (commonly referred to as VAR).. The units are VOLT_AMPERE_REACTIVE."@en .

:hasVoltAmpereReactiveValue a owl:DatatypeProperty ;
	rdfs:subPropertyOf :hasSampledValue ;
        rdfs:range xsd:float ;
	rdfs:comment "Observed result for: The measurement of reactive power in an AC electrical circuit (commonly referred to as VAR).. The units are VOLT_AMPERE_REACTIVE."@en .

:VolumeFluid a owl:Class ;
	rdfs:subClassOf :Sample ;
	rdfs:comment "The fluid volume of an object or container.. The units are MILLILITER."@en .

:hasVolumeFluidValue a owl:DatatypeProperty ;
	rdfs:subPropertyOf :hasSampledValue ;
        rdfs:range xsd:float ;
	rdfs:comment "Observed result for: The fluid volume of an object or container.. The units are MILLILITER."@en .

:ActualVolumeFluid a owl:Class ;
	rdfs:subClassOf :VolumeFluid ;
	rdfs:comment "The measured value of the data item type given by a sensor or encoder."@en .

:hasActualVolumeFluidValue a owl:DatatypeProperty ;
	rdfs:subPropertyOf :hasVolumeFluidValue ;
        rdfs:range xsd:float ;
	rdfs:comment "Observed result for: The measured value of the data item type given by a sensor or encoder."@en .

:ConsumedVolumeFluid a owl:Class ;
	rdfs:subClassOf :VolumeFluid ;
	rdfs:comment "The amount of bulk material consumed from an object or container during a manufacturing process."@en .

:hasConsumedVolumeFluidValue a owl:DatatypeProperty ;
	rdfs:subPropertyOf :hasVolumeFluidValue ;
        rdfs:range xsd:float ;
	rdfs:comment "Observed result for: The amount of bulk material consumed from an object or container during a manufacturing process."@en .

[ rdf:type owl:AllDisjointClasses ;
        owl:members (
           :ActualVolumeFluid
           :ConsumedVolumeFluid
            )
        ] .

:VolumeSpatial a owl:Class ;
	rdfs:subClassOf :Sample ;
	rdfs:comment "The geometric volume of an object or container.. The units are CUBIC_MILLIMETER."@en .

:hasVolumeSpatialValue a owl:DatatypeProperty ;
	rdfs:subPropertyOf :hasSampledValue ;
        rdfs:range xsd:float ;
	rdfs:comment "Observed result for: The geometric volume of an object or container.. The units are CUBIC_MILLIMETER."@en .

:ActualVolumeSpatial a owl:Class ;
	rdfs:subClassOf :VolumeSpatial ;
	rdfs:comment "The measured value of the data item type given by a sensor or encoder."@en .

:hasActualVolumeSpatialValue a owl:DatatypeProperty ;
	rdfs:subPropertyOf :hasVolumeSpatialValue ;
        rdfs:range xsd:float ;
	rdfs:comment "Observed result for: The measured value of the data item type given by a sensor or encoder."@en .

:ConsumedVolumeSpatial a owl:Class ;
	rdfs:subClassOf :VolumeSpatial ;
	rdfs:comment "The amount of bulk material consumed from an object or container during a manufacturing process."@en .

:hasConsumedVolumeSpatialValue a owl:DatatypeProperty ;
	rdfs:subPropertyOf :hasVolumeSpatialValue ;
        rdfs:range xsd:float ;
	rdfs:comment "Observed result for: The amount of bulk material consumed from an object or container during a manufacturing process."@en .

[ rdf:type owl:AllDisjointClasses ;
        owl:members (
           :ActualVolumeSpatial
           :ConsumedVolumeSpatial
            )
        ] .

:Wattage a owl:Class ;
	rdfs:subClassOf :Sample ;
	rdfs:comment "The measurement of power flowing through or dissipated by an electrical circuit or piece of equipment.. The units are WATT."@en .

:hasWattageValue a owl:DatatypeProperty ;
	rdfs:subPropertyOf :hasSampledValue ;
        rdfs:range xsd:float ;
	rdfs:comment "Observed result for: The measurement of power flowing through or dissipated by an electrical circuit or piece of equipment.. The units are WATT."@en .

:ActualWattage a owl:Class ;
	rdfs:subClassOf :Wattage ;
	rdfs:comment "The measured value of the data item type given by a sensor or encoder."@en .

:hasActualWattageValue a owl:DatatypeProperty ;
	rdfs:subPropertyOf :hasWattageValue ;
        rdfs:range xsd:float ;
	rdfs:comment "Observed result for: The measured value of the data item type given by a sensor or encoder."@en .

:TargetWattage a owl:Class ;
	rdfs:subClassOf :Wattage ;
	rdfs:comment "The desired measure or count for a data item value."@en .

:hasTargetWattageValue a owl:DatatypeProperty ;
	rdfs:subPropertyOf :hasWattageValue ;
        rdfs:range xsd:float ;
	rdfs:comment "Observed result for: The desired measure or count for a data item value."@en .

[ rdf:type owl:AllDisjointClasses ;
        owl:members (
           :ActualWattage
           :TargetWattage
            )
        ] .

[ rdf:type owl:AllDisjointClasses ;
        owl:members (
           :Acceleration
           :AccumulatedTime
           :Amperage
           :Angle
           :AngularAcceleration
           :AngularVelocity
           :AxisFeedrate
           :CapacityFluid
           :CapacitySpatial
           :ClockTime
           :Concentration
           :Conductivity
           :CuttingSpeed
           :Density
           :DepositionAccelerationVolumetric
           :DepositionDensity
           :DepositionMass
           :DepositionRateVolumetric
           :DepositionVolume
           :Displacement
           :ElectricalEnergy
           :EquipmentTimer
           :FillLevel
           :Flow
           :Frequency
           :GlobalPosition
           :Length
           :Level
           :LinearForce
           :Load
           :Mass
           :PathFeedrate
           :PathFeedratePerRevolution
           :PathPosition
           :PH
           :Position
           :PowerFactor
           :Pressure
           :ProcessTimer
           :Resistance
           :RotaryVelocity
           :SoundLevel
           :SpindleSpeed
           :Strain
           :Temperature
           :Tension
           :Tilt
           :Torque
           :Velocity
           :Viscosity
           :Voltage
           :VoltAmpere
           :VoltAmpereReactive
           :VolumeFluid
           :VolumeSpatial
           :Wattage
            )
        ] .

:AccelerationCondition a owl:Class ;
	rdfs:subClassOf :Condition ;
	rdfs:comment "Condition for: The measurement of the rate of change of velocity."@en .

:AccumulatedTimeCondition a owl:Class ;
	rdfs:subClassOf :Condition ;
	rdfs:comment "Condition for: The measurement of accumulated time for an activity or event."@en .

:AmperageCondition a owl:Class ;
	rdfs:subClassOf :Condition ;
	rdfs:comment "Condition for: The measurement of electrical current."@en .

:AngleCondition a owl:Class ;
	rdfs:subClassOf :Condition ;
	rdfs:comment "Condition for: The measurement of angular position."@en .

:AngularAccelerationCondition a owl:Class ;
	rdfs:subClassOf :Condition ;
	rdfs:comment "Condition for: The measurement rate of change of angular velocity."@en .

:AngularVelocityCondition a owl:Class ;
	rdfs:subClassOf :Condition ;
	rdfs:comment "Condition for: The measurement of the rate of change of angular position."@en .

:AxisFeedrateCondition a owl:Class ;
	rdfs:subClassOf :Condition ;
	rdfs:comment "Condition for: The measurement of the feedrate of a linear axis."@en .

:CapacityFluidCondition a owl:Class ;
	rdfs:subClassOf :Condition ;
	rdfs:comment "Condition for: The fluid capacity of an object or container."@en .

:CapacitySpatialCondition a owl:Class ;
	rdfs:subClassOf :Condition ;
	rdfs:comment "Condition for: The geometric capacity of an object or container."@en .

:ChuckInterlockCondition a owl:Class ;
	rdfs:subClassOf :Condition ;
	rdfs:comment "Condition for: An indication of the state of an interlock function or control logic state intended to prevent the associated chuck component from being operated."@en .

:ClockTimeCondition a owl:Class ;
	rdfs:subClassOf :Condition ;
	rdfs:comment "Condition for: The value provided by a timing device at a specific point in time."@en .

:CommunicationsCondition a owl:Class ;
	rdfs:subClassOf :Condition ;
	rdfs:comment "Condition for: An indication that the piece of equipment has experienced a communications failure."@en .

:ConcentrationCondition a owl:Class ;
	rdfs:subClassOf :Condition ;
	rdfs:comment "Condition for: The measurement of the percentage of one component within a mixture of components"@en .

:ConductivityCondition a owl:Class ;
	rdfs:subClassOf :Condition ;
	rdfs:comment "Condition for: The measurement of the ability of a material to conduct electricity."@en .

:CuttingSpeedCondition a owl:Class ;
	rdfs:subClassOf :Condition ;
	rdfs:comment "Condition for:  The speed difference (relative velocity) between the cutting mechanism and the surface of the workpiece it is operating on."@en .

:DataRangeCondition a owl:Class ;
	rdfs:subClassOf :Condition ;
	rdfs:comment "Condition for: An indication that the value of the data associated with a measured value or a calculation is outside of an expected range."@en .

:DensityCondition a owl:Class ;
	rdfs:subClassOf :Condition ;
	rdfs:comment "Condition for: The volumetric mass of a material per unit volume of that material."@en .

:DepositionAccelerationVolumetricCondition a owl:Class ;
	rdfs:subClassOf :Condition ;
	rdfs:comment "Condition for: The rate of change in spatial volume of material deposited in an additive manufacturing process."@en .

:DepositionDensityCondition a owl:Class ;
	rdfs:subClassOf :Condition ;
	rdfs:comment "Condition for: The density of the material deposited in an additive manufacturing process per unit of volume."@en .

:DepositionMassCondition a owl:Class ;
	rdfs:subClassOf :Condition ;
	rdfs:comment "Condition for: The mass of the material deposited in an additive manufacturing process."@en .

:DepositionRateVolumetricCondition a owl:Class ;
	rdfs:subClassOf :Condition ;
	rdfs:comment "Condition for: The rate at which a spatial volume of material is deposited in an additive manufacturing process."@en .

:DepositionVolumeCondition a owl:Class ;
	rdfs:subClassOf :Condition ;
	rdfs:comment "Condition for: The spatial volume of material to be deposited in an additive manufacturing process."@en .

:DirectionCondition a owl:Class ;
	rdfs:subClassOf :Condition ;
	rdfs:comment "Condition for: The direction of motion."@en .

:DisplacementCondition a owl:Class ;
	rdfs:subClassOf :Condition ;
	rdfs:comment "Condition for: The measurement of the change in position of an object."@en .

:ElectricalEnergyCondition a owl:Class ;
	rdfs:subClassOf :Condition ;
	rdfs:comment "Condition for: The measurement of electrical energy consumption by a component."@en .

:EndOfBarCondition a owl:Class ;
	rdfs:subClassOf :Condition ;
	rdfs:comment "Condition for: An indication of whether the end of a piece of bar stock being feed by a bar feeder has been reached."@en .

:EquipmentTimerCondition a owl:Class ;
	rdfs:subClassOf :Condition ;
	rdfs:comment "Condition for: The measurement of the amount of time a piece of equipment or a sub-part of a piece of equipment has performed specific activities."@en .

:FillLevelCondition a owl:Class ;
	rdfs:subClassOf :Condition ;
	rdfs:comment "Condition for: The measurement of the amount of a substance remaining compared to the planned maximum amount of that substance."@en .

:FlowCondition a owl:Class ;
	rdfs:subClassOf :Condition ;
	rdfs:comment "Condition for: The measurement of the rate of flow of a fluid."@en .

:FrequencyCondition a owl:Class ;
	rdfs:subClassOf :Condition ;
	rdfs:comment "Condition for: The measurement of the number of occurrences of a repeating event per unit time."@en .

:GlobalPositionCondition a owl:Class ;
	rdfs:subClassOf :Condition ;
	rdfs:comment "Condition for: DEPRECATED in Version 1.1"@en .

:HardwareCondition a owl:Class ;
	rdfs:subClassOf :Condition ;
	rdfs:comment "Condition for: An indication of a fault associated with the hardware subsystem of the structural element."@en .

:InterfaceStateCondition a owl:Class ;
	rdfs:subClassOf :Condition ;
	rdfs:comment "Condition for: An indication of the operational state of an interface component component."@en .

:LengthCondition a owl:Class ;
	rdfs:subClassOf :Condition ;
	rdfs:comment "Condition for: The measurement of the length of an object."@en .

:LevelCondition a owl:Class ;
	rdfs:subClassOf :Condition ;
	rdfs:comment "Condition for: DEPRECATED in Version 1.2.  See filllevel sample"@en .

:LinearForceCondition a owl:Class ;
	rdfs:subClassOf :Condition ;
	rdfs:comment "Condition for: The measurement of the push or pull introduced by an actuator or exerted on an object."@en .

:LoadCondition a owl:Class ;
	rdfs:subClassOf :Condition ;
	rdfs:comment "Condition for: The measurement of the actual versus the standard rating of a piece of equipment."@en .

:LogicProgramCondition a owl:Class ;
	rdfs:subClassOf :Condition ;
	rdfs:comment "Condition for: An indication that an error occurred in the logic program or programmable logic controller (PLC) associated with a piece of equipment."@en .

:MassCondition a owl:Class ;
	rdfs:subClassOf :Condition ;
	rdfs:comment "Condition for: The measurement of the mass of an object(s) or an amount of material."@en .

:MotionProgramCondition a owl:Class ;
	rdfs:subClassOf :Condition ;
	rdfs:comment "Condition for: An indication that an error occurred in the motion program associated with a piece of equipment."@en .

:PathFeedrateCondition a owl:Class ;
	rdfs:subClassOf :Condition ;
	rdfs:comment "Condition for: The measurement of the feedrate for the axes, or a single axis, associated with a path component-a vector."@en .

:PathFeedratePerRevolutionCondition a owl:Class ;
	rdfs:subClassOf :Condition ;
	rdfs:comment "Condition for: The feedrate for the axes, or a single axis."@en .

:PathPositionCondition a owl:Class ;
	rdfs:subClassOf :Condition ;
	rdfs:comment "Condition for: A measured or calculated position of a control point associated with a controller element, or path element if provided, of a piece of equipment."@en .

:PHCondition a owl:Class ;
	rdfs:subClassOf :Condition ;
	rdfs:comment "Condition for: A measure of the acidity or alkalinity of a solution."@en .

:PositionCondition a owl:Class ;
	rdfs:subClassOf :Condition ;
	rdfs:comment "Condition for: A measured or calculated position of a component element as reported by a piece of equipment."@en .

:PowerFactorCondition a owl:Class ;
	rdfs:subClassOf :Condition ;
	rdfs:comment "Condition for: The measurement of the ratio of real power flowing to a load to the apparent power in that AC circuit."@en .

:PressureCondition a owl:Class ;
	rdfs:subClassOf :Condition ;
	rdfs:comment "Condition for: The measurement of force per unit area exerted by a gas or liquid."@en .

:ProcessTimerCondition a owl:Class ;
	rdfs:subClassOf :Condition ;
	rdfs:comment "Condition for: The measurement of the amount of time a piece of equipment has performed different types of activities associated with the process being performed at that piece of equipment."@en .

:ResistanceCondition a owl:Class ;
	rdfs:subClassOf :Condition ;
	rdfs:comment "Condition for: The measurement of the degree to which a substance opposes the passage of an electric current."@en .

:RotaryVelocityCondition a owl:Class ;
	rdfs:subClassOf :Condition ;
	rdfs:comment "Condition for: The measurement of the rotational speed of a rotary axis."@en .

:SoundLevelCondition a owl:Class ;
	rdfs:subClassOf :Condition ;
	rdfs:comment "Condition for: The measurement of a sound level or sound pressure level relative to atmospheric pressure."@en .

:SpindleSpeedCondition a owl:Class ;
	rdfs:subClassOf :Condition ;
	rdfs:comment "Condition for: DEPRECATED in Version 1.2.  Replaced by rotaryvelocity sample"@en .

:StrainCondition a owl:Class ;
	rdfs:subClassOf :Condition ;
	rdfs:comment "Condition for: The measurement of the amount of deformation per unit length of an object when a load is applied."@en .

:SystemCondition a owl:Class ;
	rdfs:subClassOf :Condition ;
	rdfs:comment "Condition for: A general purpose indication associated with an electronic component of a piece of equipment or a controller that represents a fault that is not associated with the operator, program, or hardware."@en .

:TemperatureCondition a owl:Class ;
	rdfs:subClassOf :Condition ;
	rdfs:comment "Condition for: The measurement of temperature."@en .

:TensionCondition a owl:Class ;
	rdfs:subClassOf :Condition ;
	rdfs:comment "Condition for: The measurement of a force that stretches or elongates an object."@en .

:TiltCondition a owl:Class ;
	rdfs:subClassOf :Condition ;
	rdfs:comment "Condition for: The measurement of angular displacement. "@en .

:TorqueCondition a owl:Class ;
	rdfs:subClassOf :Condition ;
	rdfs:comment "Condition for: The measurement of the turning force exerted on an object or by an object."@en .

:VelocityCondition a owl:Class ;
	rdfs:subClassOf :Condition ;
	rdfs:comment "Condition for: The measurement of the rate of change of position of a component."@en .

:ViscosityCondition a owl:Class ;
	rdfs:subClassOf :Condition ;
	rdfs:comment "Condition for: The measurement of a fluids resistance to flow."@en .

:VoltageCondition a owl:Class ;
	rdfs:subClassOf :Condition ;
	rdfs:comment "Condition for: The measurement of electrical potential between two points."@en .

:VoltAmpereCondition a owl:Class ;
	rdfs:subClassOf :Condition ;
	rdfs:comment "Condition for: The measurement of the apparent power in an electrical circuit, equal to the product of root-mean-square (RMS) voltage and RMS current (commonly referred to as VA)."@en .

:VoltAmpereReactiveCondition a owl:Class ;
	rdfs:subClassOf :Condition ;
	rdfs:comment "Condition for: The measurement of reactive power in an AC electrical circuit (commonly referred to as VAR)."@en .

:VolumeFluidCondition a owl:Class ;
	rdfs:subClassOf :Condition ;
	rdfs:comment "Condition for: The fluid volume of an object or container."@en .

:VolumeSpatialCondition a owl:Class ;
	rdfs:subClassOf :Condition ;
	rdfs:comment "Condition for: The geometric volume of an object or container."@en .

:WattageCondition a owl:Class ;
	rdfs:subClassOf :Condition ;
	rdfs:comment "Condition for: The measurement of power flowing through or dissipated by an electrical circuit or piece of equipment."@en .

[ rdf:type owl:AllDisjointClasses ;
        owl:members (
           :AccelerationCondition
           :AccumulatedTimeCondition
           :AmperageCondition
           :AngleCondition
           :AngularAccelerationCondition
           :AngularVelocityCondition
           :AxisFeedrateCondition
           :CapacityFluidCondition
           :CapacitySpatialCondition
           :ChuckInterlockCondition
           :ClockTimeCondition
           :CommunicationsCondition
           :ConcentrationCondition
           :ConductivityCondition
           :CuttingSpeedCondition
           :DataRangeCondition
           :DensityCondition
           :DepositionAccelerationVolumetricCondition
           :DepositionDensityCondition
           :DepositionMassCondition
           :DepositionRateVolumetricCondition
           :DepositionVolumeCondition
           :DirectionCondition
           :DisplacementCondition
           :ElectricalEnergyCondition
           :EndOfBarCondition
           :EquipmentTimerCondition
           :FillLevelCondition
           :FlowCondition
           :FrequencyCondition
           :GlobalPositionCondition
           :HardwareCondition
           :InterfaceStateCondition
           :LengthCondition
           :LevelCondition
           :LinearForceCondition
           :LoadCondition
           :LogicProgramCondition
           :MassCondition
           :MotionProgramCondition
           :PathFeedrateCondition
           :PathFeedratePerRevolutionCondition
           :PathPositionCondition
           :PHCondition
           :PositionCondition
           :PowerFactorCondition
           :PressureCondition
           :ProcessTimerCondition
           :ResistanceCondition
           :RotaryVelocityCondition
           :SoundLevelCondition
           :SpindleSpeedCondition
           :StrainCondition
           :SystemCondition
           :TemperatureCondition
           :TensionCondition
           :TiltCondition
           :TorqueCondition
           :VelocityCondition
           :ViscosityCondition
           :VoltageCondition
           :VoltAmpereCondition
           :VoltAmpereReactiveCondition
           :VolumeFluidCondition
           :VolumeSpatialCondition
           :WattageCondition
            )
        ] .

